Change nominal generic terms to dispense with GVAR
This constructor is redundant (though somewhat convenient in the
λ-calculus examples) and was actively harmful in the evolving
π-calculus work.

examples/lambda/basics/nomdatatype.sig
@@ -4,7 +4,7 @@ sig
   include Abbrev
   type coninfo = {con_termP : thm, con_def : thm}
 
-  val new_type_step1 : string -> int -> thm list -> {vp:term,lp:term} ->
+  val new_type_step1 : string -> int -> thm list -> {lp:term} ->
                        {term_ABS_pseudo11 : thm,
                         term_REP_11 : thm,
                         term_REP_t : term,
