examples/lambda/basics/generic_termsScript.sml
@@ -17,12 +17,10 @@ val _ = new_theory "generic_terms";
 val _ = computeLib.auto_import_definitions := false;
 
 Datatype:
-  pregterm = var string 'v
-           | lam string (string list) 'b (pregterm list) (pregterm list)
+  pregterm = lam string (string list) 'b (pregterm list) (pregterm list)
 End
 
 Definition fv_def:
-  fv (var s vv) = {s} ∧
   fv (lam v fvs bv bndts unbndts) =
    (fvl bndts DELETE v) ∪ fvl unbndts ∪ set fvs ∧
   fvl [] = ∅ ∧
@@ -30,11 +28,10 @@ Definition fv_def:
 End
 val _ = augment_srw_ss [rewrites [fv_def]]
 
-val oldind = TypeBase.induction_of ``:(α,β)pregterm``
+val oldind = TypeBase.induction_of ``:α pregterm``
 
 Theorem pind[local]:
   ∀P.
-      (∀s vv. P (var s vv)) ∧
       (∀v bv fvs bndts unbndts.
          EVERY P bndts ∧ EVERY P unbndts ⇒ P (lam v fvs bv bndts unbndts))
     ⇒
@@ -59,7 +56,6 @@ QED
 val _ = augment_srw_ss [rewrites [finite_fv]]
 
 Definition raw_ptpm_def:
-  raw_ptpm p (var s vv) = var (lswapstr p s) vv ∧
   raw_ptpm p (lam v fvs bv bndts unbndts) =
    lam (lswapstr p v) (listpm string_pmact p fvs) bv
        (raw_ptpml p bndts) (raw_ptpml p unbndts) ∧
@@ -67,63 +63,69 @@ Definition raw_ptpm_def:
   (raw_ptpml p (h::t) = raw_ptpm p h :: raw_ptpml p t)
 End
 
-val _ = overload_on("pt_pmact",``mk_pmact raw_ptpm``);
-val _ = overload_on("ptpm",``pmact pt_pmact``);
-val _ = overload_on("ptl_pmact",``mk_pmact raw_ptpml``);
-val _ = overload_on("ptpml",``pmact ptl_pmact``);
+Overload pt_pmact = “mk_pmact raw_ptpm”
+Overload ptpm = “pmact pt_pmact”
+Overload ptl_pmact = “mk_pmact raw_ptpml”
+Overload ptpml = “pmact ptl_pmact”
 
-val raw_ptpm_nil = prove(
-  ``(∀t:(α,β)pregterm. raw_ptpm [] t = t) ∧
-    (∀l:(α,β)pregterm list. raw_ptpml [] l = l)``,
-  ho_match_mp_tac oldind >> srw_tac [][raw_ptpm_def])
+Theorem raw_ptpm_nil[local]:
+  (∀t:α pregterm. raw_ptpm [] t = t) ∧
+  (∀l:α pregterm list. raw_ptpml [] l = l)
+Proof
+  ho_match_mp_tac oldind >> srw_tac [][raw_ptpm_def]
+QED
 
-val raw_ptpm_compose = prove(
-  ``(∀t:(α,β)pregterm. raw_ptpm p1 (raw_ptpm p2 t) = raw_ptpm (p1 ++ p2) t) ∧
-    (∀l:(α,β)pregterm list.
-        raw_ptpml p1 (raw_ptpml p2 l) = raw_ptpml (p1 ++ p2) l)``,
-  ho_match_mp_tac oldind >> srw_tac [][raw_ptpm_def, pmact_decompose]);
+Theorem raw_ptpm_compose[local]:
+  (∀t:α pregterm. raw_ptpm p1 (raw_ptpm p2 t) = raw_ptpm (p1 ++ p2) t) ∧
+  (∀l:α pregterm list.
+     raw_ptpml p1 (raw_ptpml p2 l) = raw_ptpml (p1 ++ p2) l)
+Proof
+  ho_match_mp_tac oldind >> srw_tac [][raw_ptpm_def, pmact_decompose]
+QED
 
 Theorem raw_ptpm_permeq[local]:
   (∀x. lswapstr p1 x = lswapstr p2 x) ⇒
-  (∀t:(α,β)pregterm. raw_ptpm p1 t = raw_ptpm p2 t) ∧
-  (∀l:(α,β)pregterm list. raw_ptpml p1 l = raw_ptpml p2 l)
+  (∀t:α pregterm. raw_ptpm p1 t = raw_ptpm p2 t) ∧
+  (∀l:α pregterm list. raw_ptpml p1 l = raw_ptpml p2 l)
 Proof
   strip_tac >> ho_match_mp_tac oldind >> srw_tac [][raw_ptpm_def] >>
   AP_THM_TAC >> irule listpm_permeq >>
   gvs[permeq_def, stringpm_raw, FUN_EQ_THM]
 QED
 
-val ptpm_raw = prove(
-  ``(ptpm = raw_ptpm) ∧ (ptpml = raw_ptpml)``,
+Theorem ptpm_raw[local]:
+  (ptpm = raw_ptpm) ∧ (ptpml = raw_ptpml)
+Proof
   conj_tac >> (
   srw_tac [][GSYM pmact_bijections] >>
   srw_tac [][is_pmact_def] >|[
     srw_tac [][raw_ptpm_nil],
     srw_tac [][raw_ptpm_compose],
     fsrw_tac [][raw_ptpm_permeq, permeq_thm, FUN_EQ_THM]
-]));
-val ptpm_raw = INST_TYPE[gamma|->alpha,delta|->beta] ptpm_raw;
+  ])
+QED
+Theorem ptpm_raw[local,allow_rebind] = INST_TYPE[beta|->alpha] ptpm_raw
 
-val ptpml_listpm = store_thm(
-  "ptpml_listpm",
-  ``∀l. ptpml p l = listpm pt_pmact p l``,
+Theorem ptpml_listpm:
+  ∀l. ptpml p l = listpm pt_pmact p l
+Proof
   Induct >> fsrw_tac[][ptpm_raw] >>
-  srw_tac [][raw_ptpm_def]);
+  srw_tac [][raw_ptpm_def]
+QED
 
-(* |- (!p s vv. ptpm p (var s vv) = var (lswapstr p s) vv) /\
-      !p v bv bndts unbndts.
+(* |- !p v bv bndts unbndts.
         ptpm p (lam v bv bndts unbndts) =
         lam (lswapstr p v) bv (listpm pt_pmact p bndts)
           (listpm pt_pmact p unbndts)
  *)
 Theorem ptpm_thm[simp] =
-  raw_ptpm_def |> CONJUNCTS |> (fn l => List.take(l, 2))
-               |> map (SUBS (map GSYM (CONJUNCTS ptpm_raw))) |> LIST_CONJ
+  raw_ptpm_def |> CONJUNCTS |> hd
+               |> SUBS (map GSYM (CONJUNCTS ptpm_raw))
                |> REWRITE_RULE [ptpml_listpm]
 
 Theorem ptpm_fv:
-  (∀t:(α,β)pregterm. fv (ptpm p t) = ssetpm p (fv t)) ∧
-  (∀l:(α,β)pregterm list. fvl (ptpml p l) = ssetpm p (fvl l))
+  (∀t:α pregterm. fv (ptpm p t) = ssetpm p (fv t)) ∧
+  (∀l:α pregterm list. fvl (ptpml p l) = ssetpm p (fvl l))
 Proof
   ho_match_mp_tac oldind >>
   srw_tac[][stringpm_raw, ptpml_listpm, pmact_INSERT, pmact_DELETE, pmact_UNION,
@@ -132,7 +134,6 @@ QED
 val _ = augment_srw_ss [rewrites [ptpm_fv]]
 
 Definition allatoms_def:
-  (allatoms (var s vv) = {s}) ∧
   (allatoms (lam v fvs bv bndts unbndts) =
      v INSERT allatomsl bndts ∪ allatomsl unbndts ∪ set fvs) ∧
   (allatomsl [] = ∅) ∧
@@ -140,15 +141,15 @@ Definition allatoms_def:
 End
 
 Theorem allatoms_finite[simp] :
-    (∀t:(α,β)pregterm. FINITE (allatoms t)) ∧
-    (∀l:(α,β)pregterm list. FINITE (allatomsl l))
+    (∀t:α pregterm. FINITE (allatoms t)) ∧
+    (∀l:α pregterm list. FINITE (allatomsl l))
 Proof
   ho_match_mp_tac oldind >> srw_tac [][allatoms_def]
 QED
 
 Theorem allatoms_supports:
-  (∀t:(α,β)pregterm. support pt_pmact t (allatoms t)) ∧
-  (∀l:(α,β)pregterm list. support (list_pmact pt_pmact) l (allatomsl l))
+  (∀t:α pregterm. support pt_pmact t (allatoms t)) ∧
+  (∀l:α pregterm list. support (list_pmact pt_pmact) l (allatomsl l))
 Proof
   simp_tac (srw_ss())[support_def] >>
   ho_match_mp_tac oldind >> srw_tac [][allatoms_def] >>
@@ -157,10 +158,11 @@ Proof
   Induct_on ‘l’ >> simp[]
 QED
 
-val allatoms_fresh = store_thm(
-  "allatoms_fresh",
-  ``x ∉ allatoms t ∧ y ∉ allatoms t ==> (ptpm [(x,y)] t = t)``,
-  METIS_TAC [allatoms_supports, support_def]);
+Theorem allatoms_fresh:
+  x ∉ allatoms t ∧ y ∉ allatoms t ==> ptpm [(x,y)] t = t
+Proof
+  METIS_TAC [allatoms_supports, support_def]
+QED
 
 Theorem lswapstrl_apart:
   ¬MEM a l ∧ MEM b l ⇒ listpm string_pmact [(a,b)] l ≠ l
@@ -174,14 +176,15 @@ Proof
   Induct_on ‘l’ >> simp[]
 QED
 
-val allatoms_apart = store_thm(
-  "allatoms_apart",
-  ``(∀t:(α,β)pregterm a b.
-       a ∉ allatoms t /\ b ∈ allatoms t ⇒ ptpm [(a,b)] t ≠ t) ∧
-    (∀l:(α,β)pregterm list a b.
-       a ∉ allatomsl l ∧ b ∈ allatomsl l ⇒ listpm pt_pmact [(a,b)] l ≠ l)``,
+Theorem allatoms_apart:
+  (∀t:α pregterm a b.
+     a ∉ allatoms t /\ b ∈ allatoms t ⇒ ptpm [(a,b)] t ≠ t) ∧
+  (∀l:α pregterm list a b.
+     a ∉ allatomsl l ∧ b ∈ allatomsl l ⇒ listpm pt_pmact [(a,b)] l ≠ l)
+Proof
   ho_match_mp_tac oldind >> srw_tac [][allatoms_def] >>
-  metis_tac[swapstr_def, lswapstrl_apart]);
+  metis_tac[swapstr_def, lswapstrl_apart]
+QED
 
 Theorem allatoms_supp:
   supp pt_pmact t = allatoms t
@@ -197,17 +200,16 @@ Proof
   METIS_TAC [allatoms_apart]
 QED
 
-val allatoms_perm = store_thm(
-  "allatoms_perm",
-  ``(∀t:(α,β)pregterm. allatoms (ptpm p t) = ssetpm p (allatoms t)) ∧
-    (∀l:(α,β)pregterm list.
-      allatomsl (listpm pt_pmact p l) = ssetpm p (allatomsl l))``,
+Theorem allatoms_perm:
+  (∀t:α pregterm. allatoms (ptpm p t) = ssetpm p (allatoms t)) ∧
+  (∀l:α pregterm list.
+     allatomsl (listpm pt_pmact p l) = ssetpm p (allatomsl l))
+Proof
   ho_match_mp_tac oldind >>
-  srw_tac [][allatoms_def, pmact_INSERT, pmact_UNION, set_listpm]);
+  srw_tac [][allatoms_def, pmact_INSERT, pmact_UNION, set_listpm]
+QED
 
 Inductive aeq:
-[~var:]
-  (!s vv. aeq (var s vv) (var s vv))
 [~lam:]
   (!u v fvs bv z bndts1 bndts2 us1 us2.
       aeql us1 us2 ∧
@@ -220,13 +222,9 @@ Inductive aeq:
   (∀h1 h2 t1 t2. aeq h1 h2 ∧ aeql t1 t2 ⇒ aeql (h1::t1) (h2::t2))
 End
 
-Theorem aeq_distinct: ~aeq (var s vv) (lam v fvs bv ts us)
-Proof ONCE_REWRITE_TAC [aeq_cases] THEN SRW_TAC [][]
-QED
-
 Theorem aeq_ptpm_lemma:
-  (!t:(α,β)pregterm u. aeq t u ==> !p. aeq (ptpm p t) (ptpm p u)) ∧
-  (∀ts:(α,β)pregterm list us.
+  (!t:α pregterm u. aeq t u ==> !p. aeq (ptpm p t) (ptpm p u)) ∧
+  (∀ts:α pregterm list us.
       aeql ts us ⇒ ∀π. aeql (listpm pt_pmact π ts) (listpm pt_pmact π us))
 Proof
   ho_match_mp_tac aeq_ind >> srw_tac [][aeq_rules, ptpml_listpm] >>
@@ -236,34 +234,39 @@ Proof
   srw_tac [][ptpml_listpm, pmact_sing_to_back]
 QED
 
-val aeq_ptpm_eqn = store_thm(
-  "aeq_ptpm_eqn",
-  ``aeq (ptpm p t) u = aeq t (ptpm (REVERSE p) u)``,
-  METIS_TAC [aeq_ptpm_lemma, pmact_inverse]);
+Theorem aeq_ptpm_eqn:
+  aeq (ptpm p t) u = aeq t (ptpm (REVERSE p) u)
+Proof METIS_TAC [aeq_ptpm_lemma, pmact_inverse]
+QED
 
-val aeql_ptpm_eqn = store_thm(
-  "aeql_ptpm_eqn",
-  ``aeql (ptpml p l1) l2 = aeql l1 (ptpml p⁻¹ l2)``,
-  METIS_TAC [aeq_ptpm_lemma, ptpml_listpm, pmact_inverse]);
+Theorem aeql_ptpm_eqn:
+  aeql (ptpml p l1) l2 = aeql l1 (ptpml p⁻¹ l2)
+Proof METIS_TAC [aeq_ptpm_lemma, ptpml_listpm, pmact_inverse]
+QED
 
-val IN_fvl = prove(
-  ``x ∈ fvl tl ⇔ ∃e. MEM e tl ∧ x ∈ fv e``,
-  Induct_on `tl` >> srw_tac [DNF_ss][AC DISJ_ASSOC DISJ_COMM]);
+Theorem IN_fvl[local]:
+  x ∈ fvl tl ⇔ ∃e. MEM e tl ∧ x ∈ fv e
+Proof
+  Induct_on `tl` >> srw_tac [DNF_ss][AC DISJ_ASSOC DISJ_COMM]
+QED
 
-val IN_allatomsl = prove(
-  ``x ∈ allatomsl tl ⇔ ∃t. MEM t tl ∧ x ∈ allatoms t``,
-  Induct_on `tl` >> srw_tac [DNF_ss][allatoms_def]);
+Theorem IN_allatomsl[local]:
+  x ∈ allatomsl tl ⇔ ∃t. MEM t tl ∧ x ∈ allatoms t
+Proof
+  Induct_on `tl` >> srw_tac [DNF_ss][allatoms_def]
+QED
 
-val fv_SUBSET_allatoms = store_thm(
-  "fv_SUBSET_allatoms",
-  ``(∀t:(α,β)pregterm. fv t SUBSET allatoms t) ∧
-    (∀l:(α,β)pregterm list. fvl l ⊆ allatomsl l)``,
+Theorem fv_SUBSET_allatoms:
+  (∀t:α pregterm. fv t SUBSET allatoms t) ∧
+  (∀l:α pregterm list. fvl l ⊆ allatomsl l)
+Proof
   SIMP_TAC (srw_ss()) [SUBSET_DEF] >> ho_match_mp_tac oldind>>
-  srw_tac [][allatoms_def] >> metis_tac []);
+  srw_tac [][allatoms_def] >> metis_tac []
+QED
 
 Theorem aeq_fv:
-  (!t:(α,β)pregterm u. aeq t u ==> (fv t = fv u)) ∧
-  (∀ts:(α,β)pregterm list us. aeql ts us ⇒ (fvl ts = fvl us))
+  (!t:α pregterm u. aeq t u ==> (fv t = fv u)) ∧
+  (∀ts:α pregterm list us. aeql ts us ⇒ (fvl ts = fvl us))
 Proof
   ho_match_mp_tac aeq_ind >>
   srw_tac [][EXTENSION, ptpm_fv, pmact_IN, ptpml_listpm] THEN
@@ -287,7 +290,7 @@ Proof
 QED
 
 Theorem aeq_refl[simp] :
-  (∀t:(α,β)pregterm. aeq t t) ∧ (∀l:(α,β)pregterm list. aeql l l)
+  (∀t:α pregterm. aeq t t) ∧ (∀l:α pregterm list. aeql l l)
 Proof
   ho_match_mp_tac oldind >> asm_simp_tac (srw_ss())[aeq_rules] >>
   REPEAT gen_tac >> strip_tac >>
@@ -298,34 +301,30 @@ Proof
   METIS_TAC []
 QED
 
-val aeq_sym = store_thm(
-  "aeq_sym",
-  ``(∀t:(α,β)pregterm u. aeq t u ==> aeq u t) ∧
-    (∀l1:(α,β)pregterm list l2. aeql l1 l2 ==> aeql l2 l1)``,
+Theorem aeq_sym:
+  (∀t:α pregterm u. aeq t u ==> aeq u t) ∧
+  (∀l1:α pregterm list l2. aeql l1 l2 ==> aeql l2 l1)
+Proof
   ho_match_mp_tac aeq_ind >> srw_tac [][aeq_rules] >>
-  metis_tac [aeq_lam]);
+  metis_tac [aeq_lam]
+QED
 
-val aeq_var_inversion = store_thm(
-  "aeq_var_inversion",
-  ``aeq (var vv s) t = (t = var vv s)``,
-  srw_tac [][Once aeq_cases]);
-
-val aeq_lam_inversion = store_thm(
-  "aeq_lam_inversion",
-  ``aeq (lam v fvs bv bndts unbndts) N =
+Theorem aeq_lam_inversion:
+  aeq (lam v fvs bv bndts unbndts) N ⇔
       ∃z v' bndts' unbndts'.
         (N = lam v' fvs bv bndts' unbndts') ∧ z ≠ v' ∧ z ≠ v ∧
         z ∉ allatomsl bndts ∧ z ∉ allatomsl bndts' ∧
         aeql (ptpml [(v,z)] bndts) (ptpml [(v',z)] bndts') ∧
-        aeql unbndts unbndts'``,
-  srw_tac [][Once aeq_cases, SimpLHS] >> metis_tac []);
+        aeql unbndts unbndts'
+Proof
+  srw_tac [][Once aeq_cases, SimpLHS] >> metis_tac []
+QED
 
 Theorem aeq_ptm_11:
-    (aeq (var s1 vv1) (var s2 vv2) ⇔ (s1 = s2) ∧ (vv1 = vv2)) /\
     (aeq (lam v fvs1 bv1 bndts1 unbndts1) (lam v fvs2 bv2 bndts2 unbndts2) ⇔
       bv1 = bv2 ∧ fvs1 = fvs2 ∧ aeql bndts1 bndts2 ∧ aeql unbndts1 unbndts2)
 Proof
-  SRW_TAC [][aeq_lam_inversion, aeq_ptpm_eqn, aeq_var_inversion, EQ_IMP_THM]
+  SRW_TAC [][aeq_lam_inversion, aeq_ptpm_eqn, EQ_IMP_THM]
   THENL [
     full_simp_tac (srw_ss() ++ ETA_ss)
       [aeql_ptpm_eqn, pmact_nil],
@@ -340,65 +339,61 @@ val ptpml_fresh =
   allatoms_supports |> CONJUNCT2 |>
   SIMP_RULE (srw_ss()) [support_def, GSYM ptpml_listpm]
 
-val ptpml_sing_to_back' = prove(
-  ``ptpml p (ptpml [(u,v)] tl) =
-       ptpml [(lswapstr p u, lswapstr p v)] (ptpml p tl)``,
-  simp_tac (srw_ss()) [pmact_sing_to_back]);
+Theorem ptpml_sing_to_back'[local]:
+  ptpml p (ptpml [(u,v)] tl) =
+       ptpml [(lswapstr p u, lswapstr p v)] (ptpml p tl)
+Proof simp[pmact_sing_to_back]
+QED
 
 (* proof follows that on p169 of Andy Pitts, Information and Computation 186
    article: Nominal logic, a first order theory of names and binding *)
-val aeq_trans = store_thm(
-  "aeq_trans",
-  ``(∀t:(α,β)pregterm u. aeq t u ⇒ ∀v. aeq u v ==> aeq t v) ∧
-    (∀l1:(α,β)pregterm list l2. aeql l1 l2 ⇒ ∀l3. aeql l2 l3 ⇒ aeql l1 l3)``,
-  ho_match_mp_tac aeq_ind >> REPEAT conj_tac >|[
-    srw_tac [][],
-    Q_TAC SUFF_TAC
-      ‘∀u v fvs bv z bt1 bt2 ut1 (ut2:(α,β)pregterm list).
+Theorem aeq_trans:
+  (∀t:α pregterm u. aeq t u ⇒ ∀v. aeq u v ==> aeq t v) ∧
+  (∀l1:α pregterm list l2. aeql l1 l2 ⇒ ∀l3. aeql l2 l3 ⇒ aeql l1 l3)
+Proof
+  ho_match_mp_tac aeq_ind >> REPEAT conj_tac >> simp[] >~
+  [‘aeq (lam _ _ _ _ _) _ ⇒ aeq (lam _ _ _ _ _ ) _’]
+  >- (‘∀u v fvs bv z bt1 bt2 ut1 (ut2:α pregterm list).
          (∀l3. aeql (ptpml [(v,z)] bt2) l3 ⇒ aeql (ptpml [(u,z)] bt1) l3) ∧
          (∀ut3. aeql ut2 ut3 ⇒ aeql ut1 ut3) ∧
          z ∉ allatomsl bt1 ∧ z ∉ allatomsl bt2 ∧ z ≠ u ∧ z ≠ v ⇒
          ∀t3. aeq (lam v fvs bv bt2 ut2) t3 ⇒ aeq (lam u fvs bv bt1 ut1) t3’
-          >- metis_tac [] >>
-    rpt gen_tac >> strip_tac >> gen_tac >>
-    simp_tac (srw_ss()) [SimpL ``$==>``, aeq_lam_inversion] >>
-    DISCH_THEN
-      (Q.X_CHOOSE_THEN `z2`
-         (Q.X_CHOOSE_THEN `w`
-              (Q.X_CHOOSE_THEN `bt3`
-                  (Q.X_CHOOSE_THEN `ut3` STRIP_ASSUME_TAC)))) >>
-    Q_TAC (NEW_TAC "d")
-       `{z;z2;u;v;w} ∪ allatomsl bt1 ∪ allatomsl bt2 ∪ allatomsl bt3` >>
-    `∀bt3.
-       aeql (ptpml [(z,d)] (ptpml [(v,z)] bt2)) (ptpml [(z,d)] bt3) ==>
-       aeql (ptpml [(z,d)] (ptpml [(u,z)] bt1)) (ptpml [(z,d)] bt3)`
-       by FULL_SIMP_TAC (srw_ss()) [aeql_ptpm_eqn] THEN
-    POP_ASSUM
-       (Q.SPEC_THEN `ptpml [(z,d)] bt3`
-           (ASSUME_TAC o Q.GEN `bt3` o
-            SIMP_RULE (srw_ss() ++ ETA_ss)
-                      [pmact_sing_inv, pmact_nil])) THEN
-    POP_ASSUM (MP_TAC o ONCE_REWRITE_RULE [ptpml_sing_to_back']) THEN
-    SRW_TAC [][swapstr_def, ptpml_fresh] THEN
-    `aeql (ptpml [(z2,d)] (ptpml [(v,z2)] bt2))
-          (ptpml [(z2,d)] (ptpml [(w,z2)] bt3))`
-       by (srw_tac [ETA_ss]
-                   [Once aeql_ptpm_eqn, pmact_nil]) >>
-    POP_ASSUM (MP_TAC o ONCE_REWRITE_RULE [ptpml_sing_to_back']) THEN
-    SRW_TAC [][swapstr_def, ptpml_fresh] THEN
-    `aeql (ptpml [(u,d)] bt1) (ptpml [(w,d)] bt3)` by METIS_TAC [] THEN
-    METIS_TAC [aeq_lam],
+        suffices_by metis_tac [] >>
+      rpt gen_tac >> strip_tac >> gen_tac >>
+      simp_tac (srw_ss()) [SimpL “$==>”, aeq_lam_inversion] >>
+      disch_then $ qx_choosel_then[‘z2’, ‘w’, ‘bt3’, ‘ut3’] strip_assume_tac >>
+      Q_TAC (NEW_TAC "d")
+            ‘{z;z2;u;v;w} ∪ allatomsl bt1 ∪ allatomsl bt2 ∪ allatomsl bt3’ >>
+      ‘∀bt3.
+           aeql (ptpml [(z,d)] (ptpml [(v,z)] bt2)) (ptpml [(z,d)] bt3) ==>
+        aeql (ptpml [(z,d)] (ptpml [(u,z)] bt1)) (ptpml [(z,d)] bt3)’
+         by FULL_SIMP_TAC (srw_ss()) [aeql_ptpm_eqn] THEN
+        POP_ASSUM
+          (Q.SPEC_THEN ‘ptpml [(z,d)] bt3’
+            (ASSUME_TAC o Q.GEN ‘bt3’ o
+             SIMP_RULE (srw_ss() ++ ETA_ss)
+                       [pmact_sing_inv, pmact_nil])) THEN
+        POP_ASSUM (MP_TAC o ONCE_REWRITE_RULE [ptpml_sing_to_back']) THEN
+        SRW_TAC [][swapstr_def, ptpml_fresh] THEN
+        ‘aeql (ptpml [(z2,d)] (ptpml [(v,z2)] bt2))
+         (ptpml [(z2,d)] (ptpml [(w,z2)] bt3))’
+          by (srw_tac [ETA_ss]
+                      [Once aeql_ptpm_eqn, pmact_nil]) >>
+        POP_ASSUM (MP_TAC o ONCE_REWRITE_RULE [ptpml_sing_to_back']) THEN
+        SRW_TAC [][swapstr_def, ptpml_fresh] THEN
+        ‘aeql (ptpml [(u,d)] bt1) (ptpml [(w,d)] bt3)’ by METIS_TAC [] THEN
+        METIS_TAC [aeq_lam]) >~
+  [‘aeql  (_ :: _) _ ⇒ aeql (_ :: _) _’] >>
+  rpt gen_tac >> strip_tac >> gen_tac >>
+  srw_tac [][Once aeq_cases, SimpL “$==>”] >>
+  metis_tac [aeq_rules]
+QED
 
-    srw_tac [][],
-    rpt gen_tac >> strip_tac >> gen_tac >>
-    srw_tac [][Once aeq_cases, SimpL ``$==>``] >>
-    metis_tac [aeq_rules]
-  ]);
-
-val aeq_equiv = store_thm(
-  "aeq_equiv",
-  ``!t1 t2. aeq t1 t2 = (aeq t1 = aeq t2)``,
-  srw_tac [][FUN_EQ_THM] >> METIS_TAC [aeq_trans, aeq_sym, aeq_refl]);
+Theorem aeq_equiv:
+  !t1 t2. aeq t1 t2 = (aeq t1 = aeq t2)
+Proof
+  srw_tac [][FUN_EQ_THM] >> METIS_TAC [aeq_trans, aeq_sym, aeq_refl]
+QED
 
 val alt_aeq_lam = store_thm(
   "alt_aeq_lam",
@@ -412,8 +407,8 @@ val alt_aeq_lam = store_thm(
   METIS_TAC []);
 
 Theorem fresh_swap:
-  (∀t:(α,β)pregterm x y. x ∉ fv t ∧ y ∉ fv t ⇒ aeq t (ptpm [(x, y)] t)) ∧
-  (∀l:(α,β)pregterm list x y.
+  (∀t:α pregterm x y. x ∉ fv t ∧ y ∉ fv t ⇒ aeq t (ptpm [(x, y)] t)) ∧
+  (∀l:α pregterm list x y.
      x ∉ fvl l ∧ y ∉ fvl l ⇒ aeql l (ptpml [(x,y)] l))
 Proof
   ho_match_mp_tac oldind >>
@@ -499,11 +494,6 @@ val lam_respects_aeq = store_thm(
 
 val rmaeql = REWRITE_RULE [aeql_LIST_REL]
 
-val var_respects_aeq = store_thm(
-  "var_respects_aeq",
-  ``!s1 s2 vv1 vv2. (s1 = s2) ∧ (vv1 = vv2) ==> aeq (var s1 vv1) (var s2 vv2)``,
-  SRW_TAC [][]);
-
 (* ----------------------------------------------------------------------
     perform quotient!
    ---------------------------------------------------------------------- *)
@@ -530,58 +520,61 @@ val rmptpml = REWRITE_RULE [GSYM ptpml_listpm,ptpml_MAP,ptpm_raw]
 fun front n l = List.take (l, n)
 fun drop n l = List.drop(l,n)
 
-val fvl_eqrespects = prove(
-  ``∀ts1 ts2:(α,β) pregterm list. (ts1 = ts2) ==> (fvl ts1 = fvl ts2)``,
-  srw_tac [][]);
+Theorem fvl_eqrespects[local]:
+  ∀ts1 ts2:α pregterm list. (ts1 = ts2) ==> (fvl ts1 = fvl ts2)
+Proof srw_tac [][]
+QED
 
-val pregterm_size_def = definition "pregterm_size_def";
-
+val pregterm_size_thm = TypeBase.size_of “:'a pregterm”
 Definition psize_def:
-  (psize (var s vv) = 1) ∧
   (psize (lam s fvs bv ts us) =
    SUM (MAP psize ts) + SUM (MAP psize us) + LENGTH fvs + 1)
 End
 
 val psize_thm = SIMP_RULE (srw_ss()++ETA_ss) [] psize_def
 
-val psize_ptpm0 = prove(
-``(∀p:(α,β)pregterm pi. psize (ptpm pi p) = psize p) /\
-  (∀pl:(α,β)pregterm list pi. MAP psize (ptpml pi pl) = MAP psize pl)``,
-ho_match_mp_tac oldind >>
-srw_tac [][psize_thm, ptpml_listpm]);
+Theorem psize_ptpm0[local]:
+  (∀p:α pregterm pi. psize (ptpm pi p) = psize p) /\
+  (∀pl:α pregterm list pi. MAP psize (ptpml pi pl) = MAP psize pl)
+Proof
+  ho_match_mp_tac oldind >>
+  srw_tac [][psize_thm, ptpml_listpm]
+QED
 
 val psize_raw_ptpm = psize_ptpm0 |> CONJUNCT1 |> REWRITE_RULE [ptpm_raw]
 
-val psize_respects = prove(
-  ``∀t1 t2. aeq t1 t2 ⇒ (psize t1 = psize t2)``,
-qsuff_tac `(∀(t1:('a,'b) pregterm) t2. aeq t1 t2 ⇒ (psize t1 = psize t2)) ∧
-           (∀(l1:('a,'b) pregterm list) l2. aeql l1 l2 ⇒ (SUM (MAP psize l1) = SUM (MAP psize l2)))`
-  >- metis_tac [] >>
-ho_match_mp_tac aeq_ind >>
-srw_tac [][psize_thm] >>
-fsrw_tac [][psize_ptpm0]);
+Theorem psize_respects[local]:
+  ∀t1 t2. aeq t1 t2 ⇒ (psize t1 = psize t2)
+Proof
+  ‘(∀(t1:'a pregterm) t2. aeq t1 t2 ⇒ (psize t1 = psize t2)) ∧
+   (∀(l1:'a pregterm list) l2.
+      aeql l1 l2 ⇒ (SUM (MAP psize l1) = SUM (MAP psize l2)))’
+    suffices_by metis_tac [] >>
+  ho_match_mp_tac aeq_ind >>
+  srw_tac [][psize_thm] >>
+  fsrw_tac [][psize_ptpm0]
+QED
 
 val [GFV_thm0, gfvl_thm, GFV_raw_gtpm, simple_induction0,
      raw_gtpm_thm, is_pmact_raw_gtpm,
-     gterm_distinct, gterm_11,
+     gterm_11,
      GLAM_eq_thm0, FRESH_swap0,
      FINITE_GFV, gtmsize_thm, gtmsize_raw_gtpm] =
     quotient.define_quotient_types_full
     {
      types = [{name = "gterm", equiv = aeq_equiv}],
      defs = map mk_def
-       [("GLAM", ``lam:string -> string list -> α -> (α,β)pregterm list ->
-                       (α,β)pregterm list -> (α,β)pregterm``),
-        ("GVAR", ``var:string -> β -> (α,β)pregterm``),
-        ("GFV", ``fv : (α,β)pregterm -> string set``),
-        ("gfvl", ``fvl : (α,β)pregterm list -> string set``),
-        ("raw_gtpm", ``raw_ptpm : pm -> (α,β)pregterm -> (α,β)pregterm``),
-        ("gtmsize", ``psize:(α,β)pregterm ->num``)],
+       [("GLAM", ``lam:string -> string list -> α -> α pregterm list ->
+                       α pregterm list -> α pregterm``),
+        ("GFV", ``fv : α pregterm -> string set``),
+        ("gfvl", ``fvl : α pregterm list -> string set``),
+        ("raw_gtpm", ``raw_ptpm : pm -> α pregterm -> α pregterm``),
+        ("gtmsize", ``psize:α pregterm ->num``)],
      tyop_equivs = [],
      tyop_quotients = [],
      tyop_simps = [],
      respects = [rmaeql lam_respects_aeq,
-                 var_respects_aeq, CONJUNCT1 aeq_fv,
+                 CONJUNCT1 aeq_fv,
                  rmaeql (CONJUNCT2 aeq_fv),
                  aeq_ptpm_lemma
                      |> CONJUNCT1
@@ -594,28 +587,29 @@ val [GFV_thm0, gfvl_thm, GFV_raw_gtpm, simple_induction0,
                  ],
      poly_preserves = [],
      poly_respects = [],
-     old_thms = [fv_def |> CONJUNCTS |> front 2 |> LIST_CONJ,
-                 fv_def |> CONJUNCTS |> drop 2 |> LIST_CONJ,
+     old_thms = [fv_def |> CONJUNCTS |> hd,
+                 fv_def |> CONJUNCTS |> tl |> LIST_CONJ,
                  ptpm_fv', pind,
-                 ptpm_thm |> CONJUNCTS |> front 2 |> LIST_CONJ |> rmptpml,
-                 is_pmact_pmact |> Q.ISPEC `pt_pmact` |> REWRITE_RULE [ptpm_raw,is_pmact_def],
-                 aeq_distinct, rmaeql aeq_ptm_11,
+                 ptpm_thm |> rmptpml,
+                 is_pmact_pmact |> Q.ISPEC ‘pt_pmact’
+                                |> REWRITE_RULE [ptpm_raw,is_pmact_def],
+                 rmaeql aeq_ptm_11,
                  rmptpml (rmaeql lam_aeq_thm),
                  CONJUNCT1 fresh_swap |> REWRITE_RULE [ptpm_raw],
                  finite_fv,
                  psize_thm, psize_raw_ptpm]}
 
-val simple_induction = save_thm(
-  "simple_induction",
-  REWRITE_RULE [EVERY_MEM] simple_induction0)
+Theorem simple_induction =
+  REWRITE_RULE [EVERY_MEM] simple_induction0
 
-val _ = overload_on("gt_pmact",``mk_pmact raw_gtpm``);
-val _ = overload_on("gtpm",``pmact gt_pmact``);
+Overload gt_pmact = ``mk_pmact raw_gtpm``
+Overload gtpm = ``pmact gt_pmact``
 
-val gtpm_raw = store_thm(
-  "gtpm_raw",
-  ``gtpm = raw_gtpm``,
-  srw_tac [][GSYM pmact_bijections,is_pmact_def,is_pmact_raw_gtpm]);
+Theorem gtpm_raw:
+  gtpm = raw_gtpm
+Proof
+  srw_tac [][GSYM pmact_bijections,is_pmact_def,is_pmact_raw_gtpm]
+QED
 
 Theorem gtpm_thm = raw_gtpm_thm |> SUBS [GSYM gtpm_raw]
 
@@ -669,7 +663,6 @@ val gtmsize_gtpm =
 val GFV_thm = save_thm("GFV_thm", rmGFV GFV_thm0)
 val GFV_gtpm = save_thm("GFV_gtpm", rmGFV (SUBS [GSYM gtpm_raw] GFV_raw_gtpm))
 Theorem gtpm_thm[allow_rebind] = REWRITE_RULE [MAP_gtpm] gtpm_thm
-val gterm_distinct = save_thm("gterm_distinct", gterm_distinct)
 val gterm_11 = save_thm("gterm_11", gterm_11)
 val GLAM_eq_thm = save_thm("GLAM_eq_thm", rmGFV GLAM_eq_thm1)
 Theorem gtpm_fresh = rmGFV (SUBS [GSYM gtpm_raw] (GSYM FRESH_swap0))
@@ -680,15 +673,11 @@ val _ = delete_const "gfvl"
 val _ = delete_const "GFV"
 val _ = delete_const "fv"
 
-val _ = overload_on ("GFV", ``supp gt_pmact``)
-val _ = overload_on ("GFVl", ``supp (list_pmact gt_pmact)``)
-
-val _ = augment_srw_ss [rewrites [gterm_distinct]]
-
+Overload GFV = ``supp gt_pmact``
+Overload GFVl = ``supp (list_pmact gt_pmact)``
 
 (* default rewriting of negations makes a mess of these. *)
 Theorem  NOT_IN_GFV :
-  (x ∉ GFV (GVAR s vv) ⇔ x ≠ s) ∧
   (x ∉ GFV (GLAM v fvs bv ts us) ⇔
      ¬MEM x fvs ∧
      (∀u. MEM u us ⇒ x ∉ GFV u) ∧
@@ -714,18 +703,16 @@ val list_rel_split = prove(
    at the beta-value data attached to the GLAM, the number of fvs, and the
    number of arguments in the lists *)
 Inductive genind:
-[~var:]
-  ∀n:num s vv. vp n vv ==> genind vp lp n (GVAR s vv)
 [~lam:]
-  ∀n v bv ts us tns uns.
-     LIST_REL (genind vp lp) tns ts ∧
-     LIST_REL (genind vp lp) uns us ∧
+  ∀n:num v bv ts us tns uns.
+     LIST_REL (genind lp) tns ts ∧
+     LIST_REL (genind lp) uns us ∧
      lp n (LENGTH fvs) bv tns uns  ⇒
-     genind vp lp n (GLAM v fvs bv ts us)
+     genind lp n (GLAM v fvs bv ts us)
 End
 
 Theorem genind_gtpm:
-  ∀n t. genind vp lp n t ⇒ ∀pi. genind vp lp n (gtpm pi t)
+  ∀n t. genind lp n t ⇒ ∀pi. genind lp n (gtpm pi t)
 Proof
   Induct_on `genind` >>
   srw_tac [DNF_ss][gtpm_thm, genind_rules, list_rel_split] >>
@@ -735,7 +722,7 @@ Proof
 QED
 
 Theorem genind_gtpm_eqn:
-  genind vp lp n (gtpm pi t) = genind vp lp n t
+  genind lp n (gtpm pi t) = genind lp n t
 Proof
   metis_tac [pmact_inverse, genind_gtpm]
 QED
@@ -743,14 +730,14 @@ val _ = augment_srw_ss [rewrites [genind_gtpm_eqn]]
 
 val LIST_REL_genind_gtpm_eqn = store_thm(
   "LIST_REL_genind_gtpm_eqn",
-  ``LIST_REL (genind vp lp) ns (listpm gt_pmact pi ts) =
-    LIST_REL (genind vp lp) ns ts``,
+  ``LIST_REL (genind lp) ns (listpm gt_pmact pi ts) =
+    LIST_REL (genind lp) ns ts``,
   qid_spec_tac `ns` >> Induct_on `ts` >> Cases_on `ns` >>
   fsrw_tac [][]);
 
 val _ = augment_srw_ss [rewrites [FINITE_GFV, LIST_REL_genind_gtpm_eqn]]
 
-val _ = overload_on ("gtpml", ``listpm gt_pmact``)
+Overload gtpml = ``listpm gt_pmact``
 
 Theorem gtpml_eqr:
   !t u. (t = gtpml pi u) = (gtpml (REVERSE pi) t = u)
@@ -758,12 +745,12 @@ Proof srw_tac [][pmact_eql]
 QED
 
 Theorem genind_GLAM_eqn:
-  genind vp lp n (GLAM v fvs bv ts us) ⇔
-      ∃tns uns. LIST_REL (genind vp lp) tns ts ∧
-                LIST_REL (genind vp lp) uns us ∧
+  genind lp n (GLAM v fvs bv ts us) ⇔
+      ∃tns uns. LIST_REL (genind lp) tns ts ∧
+                LIST_REL (genind lp) uns us ∧
                 lp n (LENGTH fvs) bv tns uns
 Proof
-  srw_tac [DNF_ss][genind_cases, gterm_distinct, GLAM_eq_thm] >>
+  srw_tac [DNF_ss][genind_cases, GLAM_eq_thm] >>
   srw_tac [][gtpml_eqr, perm_supp] >> metis_tac []
 QED
 
@@ -774,19 +761,18 @@ QED
 Theorem bvc_genind:
   ∀P fv.
       (∀x. FINITE (fv x)) ∧
-      (∀n s vv x. vp n vv ⇒ P n (GVAR s vv) x) ∧
       (∀n v fvs bv tns uns ts us x.
-         LIST_REL (λn t. genind vp lp n t ∧ ∀x. P n t x) tns ts ∧
-         LIST_REL (λn t. genind vp lp n t ∧ ∀x. P n t x) uns us ∧
+         LIST_REL (λn t. genind lp n t ∧ ∀x. P n t x) tns ts ∧
+         LIST_REL (λn t. genind lp n t ∧ ∀x. P n t x) uns us ∧
          lp n (LENGTH fvs) bv tns uns ∧ v ∉ fv x ∧
          v ∉ supp (list_pmact gt_pmact) us
         ⇒
          P n (GLAM v fvs bv ts us) x)
    ⇒
-      ∀n t. genind vp lp n t ⇒ ∀x. P n t x
+      ∀n t. genind lp n t ⇒ ∀x. P n t x
 Proof
   rpt GEN_TAC >> strip_tac >>
-  qsuff_tac ‘∀n t. genind vp lp n t ⇒ ∀pi x. P n (gtpm pi t) x’
+  qsuff_tac ‘∀n t. genind lp n t ⇒ ∀pi x. P n (gtpm pi t) x’
   >- metis_tac [pmact_nil] >>
   Induct_on `genind` >> srw_tac [DNF_ss][gtpm_thm, list_rel_split] >>
   Q_TAC (NEW_TAC "z")
@@ -815,10 +801,9 @@ val genindX =
                |> Q.INST [`Q` |-> `P`] |> GEN_ALL
 
 val genind_KT = prove(
-  ``∀n t. genind (λn vv. T) (λn lfvs bv tns uns. T) n t``,
+  ``∀n t. genind (λn lfvs bv tns uns. T) n t``,
   CONV_TAC SWAP_FORALL_CONV >> ho_match_mp_tac simple_induction >>
-  srw_tac [][]
-  >- (match_mp_tac genind_var >> srw_tac [][]) >>
+  srw_tac [][] >>
   match_mp_tac genind_lam >>
   map_every qexists_tac [`GENLIST (K 0) (LENGTH bndts)`,
                          `GENLIST (K 0) (LENGTH unbndts)`] >>
@@ -862,15 +847,14 @@ val bvc_ind =
                       |> Q.GEN `X` |> Q.GEN `P`
 
 Theorem gterm_cases:
-  ∀t. (∃s vv. t = GVAR s vv) ∨ (∃s fvs bv ts us. t = GLAM s fvs bv ts us)
+  ∀t. ∃s fvs bv ts us. t = GLAM s fvs bv ts us
 Proof
   ho_match_mp_tac simple_induction >>
   srw_tac [][] >> metis_tac []
 QED
 
 Theorem FORALL_gterm:
-  (∀t. P t) ⇔ (∀s v. P (GVAR s v)) ∧
-              (∀s fvs bv ts us. P (GLAM s fvs bv ts us))
+  (∀t. P t) ⇔ (∀s fvs bv ts us. P (GLAM s fvs bv ts us))
 Proof
   EQ_TAC >> srw_tac [][] >>
   qspec_then `t` STRUCT_CASES_TAC gterm_cases >> srw_tac [][]
@@ -881,36 +865,33 @@ val some_5_F = prove(
   DEEP_INTRO_TAC optionTheory.some_intro THEN
   SIMP_TAC (srw_ss()) [pairTheory.FORALL_PROD, pairTheory.EXISTS_PROD]);
 
-val SUM_MAP_MEM = Q.store_thm(
-"SUM_MAP_MEM",
-`∀f x l. MEM x l ⇒ f x ≤ SUM (MAP f l)`,
-ntac 2 gen_tac >> Induct >> srw_tac [][] >>
-fsrw_tac [ARITH_ss][]);
+Theorem SUM_MAP_MEM:
+  ∀f x l. MEM x l ⇒ f x ≤ SUM (MAP f l)
+Proof
+  ntac 2 gen_tac >> Induct >> srw_tac [][] >>
+  fsrw_tac [ARITH_ss][]
+QED
 
-val vf = mk_var ("vf", ``: string -> β -> ρ -> γ``)
 val lf = mk_var ("lf", “: string -> string list -> α ->
                            (ρ -> γ) list -> (ρ -> γ) list
-                           -> (α,β)gterm list -> (α,β)gterm list -> ρ -> γ”)
+                           -> α gterm list -> α gterm list -> ρ -> γ”)
 
-val trec = “tmrec (A: string set) (ppm: ρ pmact) ^vf ^lf : (α,β)gterm -> ρ -> γ”
+val trec = “tmrec (A: string set) (ppm: ρ pmact) ^lf : α gterm -> ρ -> γ”
 
 Definition tmrec_def:
   ^trec t = λp.
-    case some(s,vv).(t = GVAR s vv) of
-      SOME (s,vv) => vf s vv p
-    | NONE => (
     case some(v,fvs,bv,ts,us).
            t = GLAM v fvs bv ts us ∧ v ∉ supp ppm p ∧ v ∉ GFVl us ∧ v ∉ A ∧
            ¬MEM v fvs
     of
       SOME (v,fvs,bv,ts,us) =>
         lf v fvs bv (MAP (^trec) ts) (MAP (^trec) us) ts us p
-    | NONE => ARB)
+    | NONE => ARB
 Termination
-  WF_REL_TAC `measure (gtmsize o SND o SND o SND o SND)` >>
+  WF_REL_TAC `measure (gtmsize o SND o SND o SND)` >>
   srw_tac [][] >>
   qspec_then `t` FULL_STRUCT_CASES_TAC gterm_cases >>
-  fsrw_tac [][some_5_F,gterm_distinct] >>
+  fsrw_tac [][some_5_F] >>
   fsrw_tac [][GLAM_eq_thm] >>
   qpat_x_assum `X = SOME Y` mp_tac >>
   DEEP_INTRO_TAC optionTheory.some_intro >>
@@ -921,10 +902,9 @@ Termination
   DECIDE_TAC
 End
 
-val vp = ``vp: num -> β -> bool``
 val lp = ``lp: num -> num -> α -> num list -> num list -> bool``
 
-val _ = temp_overload_on ("→", ``fnpm``)
+Overload "→"[local] = ``fnpm``
 val _ = temp_set_fixity "→" (Infixr 700)
 
 val relsupp_def = Define`
@@ -933,15 +913,11 @@ val relsupp_def = Define`
 `;
 
 Definition sidecond_def:
-  sidecond dpm ppm A ^vp ^lp ^vf ^lf ⇔
+  sidecond dpm ppm A ^lp ^lf ⇔
   FINITE A ∧ (∀p. FINITE (supp ppm p)) ∧
-    (∀x y s vv n p.
-       x ∉ A ∧ y ∉ A ∧ genind vp lp n (GVAR s vv) ⇒
-       (pmact dpm [(x,y)] (^vf s vv p) =
-        ^vf (lswapstr [(x,y)] s) vv (pmact ppm [(x,y)] p))) ∧
     (∀x y n v fvs bv r1 r2 ts us p.
        x ∉ A ∧ y ∉ A ∧ v ∉ A ∧
-       genind vp lp n (GLAM v fvs bv ts us) ∧
+       genind lp n (GLAM v fvs bv ts us) ∧
        LIST_REL (relsupp A dpm ppm) ts r1 ∧
        LIST_REL (relsupp A dpm ppm) us r2 ∧
        v ∉ supp ppm p ⇒
@@ -957,13 +933,13 @@ Definition sidecond_def:
 End
 
 val FCB_def = Define`
-  FCB dpm ppm A ^vp ^lp ^lf ⇔
+  FCB dpm ppm A ^lp ^lf ⇔
   ∀a n v fvs bv r1 r2 ts us p.
      a ∉ A ∧ a ∉ GFVl us ∧ a ∉ supp ppm p ∧
      ¬MEM a fvs ∧
      LIST_REL (relsupp A dpm ppm) ts r1 ∧
      LIST_REL (relsupp A dpm ppm) us r2 ∧
-     genind vp lp n (GLAM v fvs bv ts us) ⇒
+     genind lp n (GLAM v fvs bv ts us) ⇒
      a ∉ supp dpm (^lf a fvs bv r1 r2 ts us p)`
 
 val some_2_EQ = prove(
@@ -976,18 +952,9 @@ val some_2_F = prove(
   DEEP_INTRO_TAC optionTheory.some_intro THEN
   SIMP_TAC (srw_ss()) [pairTheory.FORALL_PROD, pairTheory.EXISTS_PROD]);
 
-val tmrec_GVAR = tmrec_def |> SPEC_ALL |> Q.INST [`t` |-> `GVAR s vv`]
-  |> SIMP_RULE (srw_ss()++ETA_ss) [gterm_11,some_2_EQ]
 val tmrec_GLAM = tmrec_def |> SPEC_ALL |> Q.INST [`t` |-> `GLAM v fvs bv ts us`]
-  |> SIMP_RULE (srw_ss()) [gterm_distinct,some_2_F,NOT_IN_supp_listpm]
+  |> SIMP_RULE (srw_ss()) [some_2_F,NOT_IN_supp_listpm]
   |> C (foldr (uncurry Q.GEN)) [`v`,‘fvs’, `bv`,`ts`,`us`]
-
-val gtpm_GVAR = gtpm_thm |> CONJUNCT1
-val genind_GVAR = store_thm(
-  "genind_GVAR",
-  ``genind vp lp n (GVAR s vv) = vp n vv``,
-  srw_tac [][genind_cases,gterm_distinct,gterm_11]);
-val GFV_GVAR = GFV_thm |> CONJUNCT1
 
 Theorem gtpm_eqr:
   (t = gtpm pi u) = (gtpm (REVERSE pi) t = u)
@@ -1001,22 +968,25 @@ val trec_fnpm = prove(
     λp. pmact apm π (tmrec A ppm vf lf t (pmact ppm π⁻¹ p))``,
   srw_tac [][FUN_EQ_THM, fnpm_def]);
 
-val MAP_trec_fnpm = prove(
-``MAP ((ppm → dpm) pi o tmrec A ppm vf lf)=
-  MAP (λt p. pmact dpm pi (tmrec A ppm vf lf t (pmact ppm (REVERSE pi) p)))``,
-ONCE_REWRITE_TAC [FUN_EQ_THM] >>
-Induct >> srw_tac [][trec_fnpm]);
+Theorem MAP_trec_fnpm[local]:
+  MAP ((ppm → dpm) pi o tmrec A ppm vf lf) =
+  MAP (λt p. pmact dpm pi (tmrec A ppm vf lf t (pmact ppm (REVERSE pi) p)))
+Proof
+  ONCE_REWRITE_TAC [FUN_EQ_THM] >>
+  Induct >> srw_tac [][trec_fnpm]
+QED
 
-val genind_GLAM_subterm = store_thm(
-"genind_GLAM_subterm",
-``genind vp lp n (GLAM v fvs bv ts us) ∧ (MEM u ts ∨ MEM u us) ⇒
-    ∃n. genind vp lp n u``,
-srw_tac [][Once genind_cases,gterm_distinct] >>
-fsrw_tac [][GLAM_eq_thm] >>
-fsrw_tac [][LIST_REL_EL_EQN,MEM_EL] >>
-srw_tac [][] >>
-fsrw_tac [][EL_MAP] >>
-metis_tac []);
+Theorem genind_GLAM_subterm:
+  genind lp n (GLAM v fvs bv ts us) ∧ (MEM u ts ∨ MEM u us) ⇒
+  ∃n. genind lp n u
+Proof
+  srw_tac [][Once genind_cases] >>
+  fsrw_tac [][GLAM_eq_thm] >>
+  fsrw_tac [][LIST_REL_EL_EQN,MEM_EL] >>
+  srw_tac [][] >>
+  fsrw_tac [][EL_MAP] >>
+  metis_tac []
+QED
 
 val gtmsize_GLAM_subterm = store_thm(
 "gtmsize_GLAM_subterm",
@@ -1026,17 +996,19 @@ imp_res_tac SUM_MAP_MEM >>
 pop_assum (qspec_then `gtmsize` mp_tac) >>
 DECIDE_TAC);
 
-val LIST_REL_relsupp_gtpml = prove(
-  ``∀A dpm ppm l1 l2.
+Theorem LIST_REL_relsupp_gtpml[local]:
+  ∀A dpm ppm l1 l2.
       LIST_REL (relsupp A dpm ppm) l1 l2 ==>
       ∀x y. x ∉ A ∧ y ∉ A ==>
          LIST_REL (relsupp A dpm ppm)
                   (gtpml [(x,y)] l1)
-                  (listpm (fn_pmact ppm dpm) [(x,y)] l2)``,
+                  (listpm (fn_pmact ppm dpm) [(x,y)] l2)
+Proof
   ntac 3 gen_tac >>
   Induct_on `LIST_REL` >> srw_tac [][relsupp_def, fnpm_def, perm_supp] >>
   first_x_assum match_mp_tac >> srw_tac [][perm_supp] >>
-  srw_tac [][swapstr_def])
+  srw_tac [][swapstr_def]
+QED
 
 fun ih_commute_tac dir (asl,w) =
     first_x_assum (fn rwt =>
@@ -1045,7 +1017,7 @@ fun ih_commute_tac dir (asl,w) =
          else NO_TAC) (asl,w)
 
 fun sidecond_tac dir =
-  qpat_x_assum `sidecond AA BB CC DD EE FF GG`
+  qpat_x_assum `sidecond AA BB CC DD EE `
      (fn th => th |> SIMP_RULE (srw_ss()) [sidecond_def] |> CONJUNCTS
                   |> last |> (fn th' => assume_tac th >> assume_tac th')) >>
   (fn (asl,w) =>
@@ -1061,40 +1033,35 @@ val listpm_tMAP = prove(
 val _ = temp_delsimps ["lift_disj_eq", "lift_imp_disj"]
 
 Theorem genind_ignores_fvspm:
-  genind vp lp n (GLAM v (listpm string_pmact pi fvs) bv ts us) ⇔
-  genind vp lp n (GLAM v fvs bv ts us)
+  genind lp n (GLAM v (listpm string_pmact pi fvs) bv ts us) ⇔
+  genind lp n (GLAM v fvs bv ts us)
 Proof
   simp[genind_GLAM_eqn]
 QED
 
 Theorem tmrec_equivariant:
-  sidecond dpm ppm A ^vp ^lp ^vf ^lf ∧ FCB dpm ppm A ^vp ^lp ^lf ⇒
-  ∀n. genind vp lp n t ⇒
+  sidecond dpm ppm A ^lp ^lf ∧ FCB dpm ppm A ^lp ^lf ⇒
+  ∀n. genind lp n t ⇒
       ∀p x y. x ∉ A ∧ y ∉ A ⇒
-        (pmact dpm [(x,y)] (tmrec A ppm vf lf t p) =
-         tmrec A ppm vf lf (gtpm [(x,y)] t) (pmact ppm [(x,y)] p))
+              (pmact dpm [(x,y)] (tmrec A ppm lf t p) =
+               tmrec A ppm lf (gtpm [(x,y)] t) (pmact ppm [(x,y)] p))
 Proof
-strip_tac >>
-completeInduct_on ‘gtmsize t’ >>
-qabbrev_tac ‘m = v’ >> markerLib.RM_ALL_ABBREVS_TAC >>
-pop_assum (strip_assume_tac o SIMP_RULE (srw_ss() ++ DNF_ss) []) >>
-simp_tac (srw_ss()) [Once FORALL_gterm] >>
-conj_tac >- (
-  (* GVAR case *)
-  srw_tac [][gtpm_GVAR,tmrec_GVAR] >>
-  fsrw_tac [][sidecond_def] >>
-  metis_tac [lswapstr_sing]) >>
-rpt gen_tac >>
-disch_then SUBST_ALL_TAC >>
-gen_tac >> strip_tac >>
-qx_gen_tac ‘p’ >>
-Q.SPECL_THEN [‘s’,‘fvs’, ‘bv’,‘ts’,‘us’,‘p’] MP_TAC
-  (tmrec_GLAM |> SIMP_RULE (srw_ss()) [FUN_EQ_THM]) >>
-DEEP_INTRO_TAC optionTheory.some_intro >>
-asm_simp_tac (srw_ss()) [pairTheory.FORALL_PROD] >>
-‘FINITE A ∧ (∀p. FINITE (supp ppm p))’
-   by fsrw_tac [][sidecond_def] >>
-reverse conj_tac >- (
+  strip_tac >>
+  completeInduct_on ‘gtmsize t’ >>
+  qabbrev_tac ‘m = v’ >> markerLib.RM_ALL_ABBREVS_TAC >>
+  pop_assum (strip_assume_tac o SIMP_RULE (srw_ss() ++ DNF_ss) []) >>
+  simp_tac (srw_ss()) [Once FORALL_gterm] >>
+  rpt gen_tac >>
+  disch_then SUBST_ALL_TAC >>
+  gen_tac >> strip_tac >>
+  qx_gen_tac ‘p’ >>
+  Q.SPECL_THEN [‘s’,‘fvs’, ‘bv’,‘ts’,‘us’,‘p’] MP_TAC
+   (tmrec_GLAM |> SIMP_RULE (srw_ss()) [FUN_EQ_THM]) >>
+  DEEP_INTRO_TAC optionTheory.some_intro >>
+  asm_simp_tac (srw_ss()) [pairTheory.FORALL_PROD] >>
+  ‘FINITE A ∧ (∀p. FINITE (supp ppm p))’
+    by fsrw_tac [][sidecond_def] >>
+  reverse conj_tac >- (
   (* bogus some(...) = ARB case *)
   Q_TAC (NEW_TAC "z") ‘supp ppm p ∪ A ∪ GFVl us ∪ GFVl ts ∪ {s} ∪ set fvs’ >>
   disch_then (qspec_then ‘z’ mp_tac) >>
@@ -1102,19 +1069,19 @@ reverse conj_tac >- (
                [GLAM_eq_thm,IN_GFVl,gtpml_eqr,listpm_MAP,MEM_MAP,GFV_gtpm] >>
   fsrw_tac [][IN_GFVl] >>
   metis_tac []) >>
-map_every qx_gen_tac [‘s'’,‘fvs'’, ‘bv'’,‘ts'’,‘us'’] >>
-strip_tac >>
-strip_tac >>
-‘fvs' = fvs ∧ us' = us ∧ bv' = bv’
-  by fsrw_tac [][GLAM_eq_thm] >> rpt VAR_EQ_TAC >>
-asm_simp_tac (srw_ss()++DNF_ss) [gtpm_thm,IN_GFVl,GFV_thm] >>
-map_every qx_gen_tac [‘x’, ‘y’] >>
-strip_tac >>
-qpat_x_assum ‘tmrec A ppm vf lf (GLAM X _ Y Z WW) p = XX’ (K ALL_TAC) >>
-srw_tac [][tmrec_GLAM] >>
-DEEP_INTRO_TAC optionTheory.some_intro >>
-asm_simp_tac (srw_ss()++ETA_ss) [pairTheory.FORALL_PROD] >>
-reverse conj_tac >- (
+  map_every qx_gen_tac [‘s'’,‘fvs'’, ‘bv'’,‘ts'’,‘us'’] >>
+  strip_tac >>
+  strip_tac >>
+  ‘fvs' = fvs ∧ us' = us ∧ bv' = bv’
+    by fsrw_tac [][GLAM_eq_thm] >> rpt VAR_EQ_TAC >>
+  asm_simp_tac (srw_ss()++DNF_ss) [gtpm_thm,IN_GFVl,GFV_thm] >>
+  map_every qx_gen_tac [‘x’, ‘y’] >>
+  strip_tac >>
+  qpat_x_assum ‘tmrec A ppm lf (GLAM X _ Y Z WW) p = XX’ (K ALL_TAC) >>
+  srw_tac [][tmrec_GLAM] >>
+  DEEP_INTRO_TAC optionTheory.some_intro >>
+  asm_simp_tac (srw_ss()++ETA_ss) [pairTheory.FORALL_PROD] >>
+  reverse conj_tac >- (
   (* bogus ARB case *)
   asm_simp_tac (srw_ss()) [GLAM_eq_thm] >>
   Q_TAC (NEW_TAC "z")
@@ -1126,109 +1093,109 @@ reverse conj_tac >- (
   reverse conj_tac >- metis_tac [] >>
   conj_tac >- metis_tac [] >>
   srw_tac [][] >> metis_tac []) >>
-qabbrev_tac ‘r1 = MAP (tmrec A ppm vf lf) ts'’ >>
-qabbrev_tac ‘r2 = MAP (tmrec A ppm vf lf) us’ >>
-fsrw_tac [][AND_IMP_INTRO] >>
-‘∃tns uns. LIST_REL (genind vp lp) tns ts ∧ LIST_REL (genind vp lp) uns us’
-  by (fsrw_tac [][genind_cases, GLAM_eq_thm] >> srw_tac [][] >>
-      metis_tac []) >>
-‘LIST_REL (genind vp lp) tns ts'’
-   by (fsrw_tac [][GLAM_eq_thm] >> srw_tac [][] >> fsrw_tac [][]) >>
-qabbrev_tac ‘GGSIZE = gtmsize (GLAM s' fvs bv ts' us)’ >>
-‘∀t n' a. gtmsize t < GGSIZE ∧ genind vp lp n' t ∧ a ∉ A ∧ a ∉ GFV t ==>
-          a ∉ supp (fn_pmact ppm dpm) (tmrec A ppm vf lf t)’
-   by (srw_tac [][] >> match_mp_tac notinsupp_I >>
-       qexists_tac ‘A ∪ GFV t’ >>
-       srw_tac [][support_def, fnpm_def, FUN_EQ_THM] >>
-       metis_tac [supp_fresh, pmact_sing_inv]) >>
-‘LIST_REL (relsupp A dpm ppm) ts' r1 ∧ LIST_REL (relsupp A dpm ppm) us r2’
-  by (srw_tac [][LIST_REL_EL_EQN, relsupp_def, Abbr‘r1’, Abbr‘r2’] >>
-      srw_tac [][EL_MAP] >> first_x_assum match_mp_tac >|
-      [qexists_tac ‘EL n' tns’, qexists_tac ‘EL n' uns’] >>
-      metis_tac [LIST_REL_EL_EQN, MEM_EL, gtmsize_GLAM_subterm]) >>
-(* COMPLETE THIS... *)
-‘∀t p x y.
-   (MEM t ts' ∨ MEM t us ∨ MEM t ts) ∧ x ∉ A ∧ y ∉ A ==>
-   (pmact dpm [(x,y)] (tmrec A ppm vf lf t p) =
-      tmrec A ppm vf lf (gtpm [(x,y)] t) (pmact ppm [(x,y)] p))’
-   by (srw_tac [][] >> first_x_assum match_mp_tac >>
-       fsrw_tac [][GLAM_eq_thm] >> srw_tac [][] >>
-       fsrw_tac [][MEM_listpm_EXISTS, gtmsize_gtpm] >>
-       metis_tac [genind_GLAM_subterm, gtmsize_GLAM_subterm]) >>
-(* THEN COMPLETE THIS ... *)
-‘(∀a b. a ∉ A ∧ b ∉ A ==>
-        (listpm (fn_pmact ppm dpm) [(a,b)] r1 =
-         MAP (tmrec A ppm vf lf) (gtpml [(a,b)] ts'))) ∧
- (∀a b. a ∉ A ∧ b ∉ A ==>
-        (listpm (fn_pmact ppm dpm) [(a,b)] r2 =
-         MAP (tmrec A ppm vf lf) (gtpml [(a,b)] us)))’
-  by (asm_simp_tac (srw_ss() ++ DNF_ss)
-                   [listpm_tMAP, MAP_EQ_f, MEM_listpm_EXISTS,
-                    Abbr‘r1’, Abbr‘r2’, fnpm_def, FUN_EQ_THM,
-                    pmact_sing_inv]) >>
-map_every qx_gen_tac [‘s''’, ‘fvs'’, ‘bv'’, ‘ts''’, ‘us'’] >>
-srw_tac [][] >>
-‘fvs' = listpm string_pmact [(x,y)] fvs ∧ bv' = bv ∧ us' = gtpml [(x,y)] us’
-  by fsrw_tac [][GLAM_eq_thm] >>
-rpt VAR_EQ_TAC >>
-sidecond_tac lhs >>
-disch_then (fn th => asm_simp_tac (srw_ss()) [th]) >>
-qpat_x_assum ‘GLAM (swapstr x y s') _ bv Z1 Z2 = Z3’ mp_tac >>
-srw_tac [][GLAM_eq_thm] >>
-qabbrev_tac ‘u = swapstr x y s'’ >>
-fsrw_tac [][gtpml_eqr] >>
-qpat_x_assum ‘XX = ts''’ (SUBST_ALL_TAC o SYM) >>
-‘u ∉ A’ by srw_tac [][Abbr‘u’,swapstr_def] >>
-‘u ∉ supp ppm (pmact ppm [(x,y)] p)’ by srw_tac [][Abbr‘u’,perm_supp] >>
-‘s'' ∉ supp (list_pmact gt_pmact) (gtpml [(x,y)] us) ∧
- s'' ∉ supp (list_pmact gt_pmact) (gtpml [(x,y)] ts')’ by (
-  fsrw_tac [DNF_ss][IN_GFVl,listpm_MAP,MEM_MAP,GFV_gtpm] >>
-  metis_tac [] ) >>
-‘u ∉ supp (list_pmact gt_pmact) (gtpml [(x,y)] us)’ by (
-  fsrw_tac [DNF_ss][IN_GFVl,listpm_MAP,MEM_MAP,GFV_gtpm,Abbr‘u’] >>
-  metis_tac [] ) >>
-‘genind vp lp n
+  qabbrev_tac ‘r1 = MAP (tmrec A ppm lf) ts'’ >>
+  qabbrev_tac ‘r2 = MAP (tmrec A ppm lf) us’ >>
+  fsrw_tac [][AND_IMP_INTRO] >>
+  ‘∃tns uns. LIST_REL (genind lp) tns ts ∧ LIST_REL (genind lp) uns us’
+    by (fsrw_tac [][genind_cases, GLAM_eq_thm] >> srw_tac [][] >>
+        metis_tac []) >>
+  ‘LIST_REL (genind lp) tns ts'’
+    by (fsrw_tac [][GLAM_eq_thm] >> srw_tac [][] >> fsrw_tac [][]) >>
+  qabbrev_tac ‘GGSIZE = gtmsize (GLAM s' fvs bv ts' us)’ >>
+  ‘∀t n' a. gtmsize t < GGSIZE ∧ genind lp n' t ∧ a ∉ A ∧ a ∉ GFV t ==>
+            a ∉ supp (fn_pmact ppm dpm) (tmrec A ppm lf t)’
+    by (srw_tac [][] >> match_mp_tac notinsupp_I >>
+        qexists_tac ‘A ∪ GFV t’ >>
+        srw_tac [][support_def, fnpm_def, FUN_EQ_THM] >>
+        metis_tac [supp_fresh, pmact_sing_inv]) >>
+  ‘LIST_REL (relsupp A dpm ppm) ts' r1 ∧ LIST_REL (relsupp A dpm ppm) us r2’
+    by (srw_tac [][LIST_REL_EL_EQN, relsupp_def, Abbr‘r1’, Abbr‘r2’] >>
+        srw_tac [][EL_MAP] >> first_x_assum match_mp_tac >|
+        [qexists_tac ‘EL n' tns’, qexists_tac ‘EL n' uns’] >>
+        metis_tac [LIST_REL_EL_EQN, MEM_EL, gtmsize_GLAM_subterm]) >>
+  (* COMPLETE THIS... *)
+  ‘∀t p x y.
+     (MEM t ts' ∨ MEM t us ∨ MEM t ts) ∧ x ∉ A ∧ y ∉ A ==>
+     (pmact dpm [(x,y)] (tmrec A ppm lf t p) =
+      tmrec A ppm lf (gtpm [(x,y)] t) (pmact ppm [(x,y)] p))’
+    by (srw_tac [][] >> first_x_assum match_mp_tac >>
+        fsrw_tac [][GLAM_eq_thm] >> srw_tac [][] >>
+        fsrw_tac [][MEM_listpm_EXISTS, gtmsize_gtpm] >>
+        metis_tac [genind_GLAM_subterm, gtmsize_GLAM_subterm]) >>
+  (* THEN COMPLETE THIS ... *)
+  ‘(∀a b. a ∉ A ∧ b ∉ A ==>
+          (listpm (fn_pmact ppm dpm) [(a,b)] r1 =
+           MAP (tmrec A ppm lf) (gtpml [(a,b)] ts'))) ∧
+   (∀a b. a ∉ A ∧ b ∉ A ==>
+          (listpm (fn_pmact ppm dpm) [(a,b)] r2 =
+           MAP (tmrec A ppm lf) (gtpml [(a,b)] us)))’
+    by (asm_simp_tac (srw_ss() ++ DNF_ss)
+                     [listpm_tMAP, MAP_EQ_f, MEM_listpm_EXISTS,
+                      Abbr‘r1’, Abbr‘r2’, fnpm_def, FUN_EQ_THM,
+                      pmact_sing_inv]) >>
+  map_every qx_gen_tac [‘s''’, ‘fvs'’, ‘bv'’, ‘ts''’, ‘us'’] >>
+  srw_tac [][] >>
+  ‘fvs' = listpm string_pmact [(x,y)] fvs ∧ bv' = bv ∧ us' = gtpml [(x,y)] us’
+    by fsrw_tac [][GLAM_eq_thm] >>
+  rpt VAR_EQ_TAC >>
+  sidecond_tac lhs >>
+  disch_then (fn th => asm_simp_tac (srw_ss()) [th]) >>
+  qpat_x_assum ‘GLAM (swapstr x y s') _ bv Z1 Z2 = Z3’ mp_tac >>
+  srw_tac [][GLAM_eq_thm] >>
+  qabbrev_tac ‘u = swapstr x y s'’ >>
+  fsrw_tac [][gtpml_eqr] >>
+  qpat_x_assum ‘XX = ts''’ (SUBST_ALL_TAC o SYM) >>
+  ‘u ∉ A’ by srw_tac [][Abbr‘u’,swapstr_def] >>
+  ‘u ∉ supp ppm (pmact ppm [(x,y)] p)’ by srw_tac [][Abbr‘u’,perm_supp] >>
+  ‘s'' ∉ supp (list_pmact gt_pmact) (gtpml [(x,y)] us) ∧
+   s'' ∉ supp (list_pmact gt_pmact) (gtpml [(x,y)] ts')’ by (
+    fsrw_tac [DNF_ss][IN_GFVl,listpm_MAP,MEM_MAP,GFV_gtpm] >>
+    metis_tac [] ) >>
+  ‘u ∉ supp (list_pmact gt_pmact) (gtpml [(x,y)] us)’ by (
+    fsrw_tac [DNF_ss][IN_GFVl,listpm_MAP,MEM_MAP,GFV_gtpm,Abbr‘u’] >>
+    metis_tac [] ) >>
+  ‘genind lp n
    (GLAM u (listpm string_pmact[(x,y)] fvs) bv
          (gtpml [(x,y)] ts') (gtpml [(x,y)] us))’ by (
-  qmatch_abbrev_tac ‘genind vp lp n t’ >>
-  qsuff_tac ‘t = gtpm [(x,y)] (GLAM s' fvs bv ts' us)’ >- srw_tac [][] >>
-  srw_tac [][Abbr‘t’,gtpm_thm] ) >>
-qmatch_abbrev_tac ‘LHS = RHS’ >>
-match_mp_tac EQ_TRANS >>
-qexists_tac ‘pmact dpm [(u,s'')] RHS’ >>
-qabbrev_tac ‘usxyts = gtpml [(u,s'')] (gtpml [(x,y)] ts')’ >>
-qabbrev_tac ‘xyus = gtpml [(x,y)] us’ >>
-qabbrev_tac ‘usxyfvs = listpm string_pmact [(u,s'')] $
-                       listpm string_pmact [(x,y)] fvs’ >>
-‘genind vp lp n (GLAM s'' usxyfvs bv usxyts xyus)’
-  by(first_x_assum (mp_tac o MATCH_MP genind_gtpm) >>
-     disch_then (qspec_then ‘[(u,s'')]’ mp_tac) >>
-     CONV_TAC (LAND_CONV (RAND_CONV (REWRITE_CONV [gtpm_thm]))) >>
-     asm_simp_tac (srw_ss()) [supp_fresh]) >>
-‘genind vp lp n (GLAM s'' fvs bv usxyts xyus)’
-  by gvs[Abbr‘usxyfvs’, genind_ignores_fvspm] >>
-‘LIST_REL (relsupp A dpm ppm) usxyts (MAP (tmrec A ppm vf lf) usxyts) ∧
- LIST_REL (relsupp A dpm ppm) xyus (MAP (tmrec A ppm vf lf) xyus)’
-   by (map_every qunabbrev_tac [‘r1’, ‘r2’, ‘usxyts’, ‘xyus’] >>
-       rpt (first_x_assum (mp_tac o MATCH_MP LIST_REL_relsupp_gtpml)) >>
-       rpt (disch_then (qspecl_then [‘x’,‘y’] assume_tac)) >>
-       ntac 2 (pop_assum mp_tac) >> asm_simp_tac (srw_ss()) [] >>
-       rpt (disch_then (assume_tac o MATCH_MP LIST_REL_relsupp_gtpml)) >>
-       ntac 2 (pop_assum (qspecl_then [‘u’, ‘s''’] mp_tac)) >>
-       asm_simp_tac (srw_ss()) [listpm_tMAP] >>
-       rpt (disch_then assume_tac) >>
-       qpat_x_assum ‘LIST_REL _ (_ (_ ts')) (MAP _ _)’ mp_tac >>
-       qmatch_abbrev_tac
+    qmatch_abbrev_tac ‘genind lp n t’ >>
+    qsuff_tac ‘t = gtpm [(x,y)] (GLAM s' fvs bv ts' us)’ >- srw_tac [][] >>
+    srw_tac [][Abbr‘t’,gtpm_thm] ) >>
+  qmatch_abbrev_tac ‘LHS = RHS’ >>
+  match_mp_tac EQ_TRANS >>
+  qexists_tac ‘pmact dpm [(u,s'')] RHS’ >>
+  qabbrev_tac ‘usxyts = gtpml [(u,s'')] (gtpml [(x,y)] ts')’ >>
+  qabbrev_tac ‘xyus = gtpml [(x,y)] us’ >>
+  qabbrev_tac ‘usxyfvs = listpm string_pmact [(u,s'')] $
+                                listpm string_pmact [(x,y)] fvs’ >>
+  ‘genind lp n (GLAM s'' usxyfvs bv usxyts xyus)’
+    by(first_x_assum (mp_tac o MATCH_MP genind_gtpm) >>
+       disch_then (qspec_then ‘[(u,s'')]’ mp_tac) >>
+       CONV_TAC (LAND_CONV (RAND_CONV (REWRITE_CONV [gtpm_thm]))) >>
+       asm_simp_tac (srw_ss()) [supp_fresh]) >>
+  ‘genind lp n (GLAM s'' fvs bv usxyts xyus)’
+    by gvs[Abbr‘usxyfvs’, genind_ignores_fvspm] >>
+  ‘LIST_REL (relsupp A dpm ppm) usxyts (MAP (tmrec A ppm lf) usxyts) ∧
+   LIST_REL (relsupp A dpm ppm) xyus (MAP (tmrec A ppm lf) xyus)’
+    by (map_every qunabbrev_tac [‘r1’, ‘r2’, ‘usxyts’, ‘xyus’] >>
+        rpt (first_x_assum (mp_tac o MATCH_MP LIST_REL_relsupp_gtpml)) >>
+        rpt (disch_then (qspecl_then [‘x’,‘y’] assume_tac)) >>
+        ntac 2 (pop_assum mp_tac) >> asm_simp_tac (srw_ss()) [] >>
+        rpt (disch_then (assume_tac o MATCH_MP LIST_REL_relsupp_gtpml)) >>
+        ntac 2 (pop_assum (qspecl_then [‘u’, ‘s''’] mp_tac)) >>
+        asm_simp_tac (srw_ss()) [listpm_tMAP] >>
+        rpt (disch_then assume_tac) >>
+        qpat_x_assum ‘LIST_REL _ (_ (_ ts')) (MAP _ _)’ mp_tac >>
+        qmatch_abbrev_tac
         ‘LIST_REL RR TS (MAP f1 TS) ==> LIST_REL RR TS (MAP f2 TS)’ >>
-       qsuff_tac ‘MAP f1 TS = MAP f2 TS’ >- srw_tac [][] >>
-       srw_tac [][MAP_EQ_f] >>
-       map_every qunabbrev_tac [‘f1’, ‘f2’, ‘TS’] >>
-       asm_simp_tac (srw_ss()) [FUN_EQ_THM, fnpm_def] >> gen_tac >>
-       ih_commute_tac lhs >> asm_simp_tac (srw_ss()) [pmact_sing_inv] >>
-       disch_then match_mp_tac >>
-       fsrw_tac [][MEM_listpm_EXISTS, gtmsize_gtpm] >>
-       metis_tac [gtmsize_GLAM_subterm, genind_GLAM_subterm]) >>
-reverse conj_tac >- (
+        qsuff_tac ‘MAP f1 TS = MAP f2 TS’ >- srw_tac [][] >>
+        srw_tac [][MAP_EQ_f] >>
+        map_every qunabbrev_tac [‘f1’, ‘f2’, ‘TS’] >>
+        asm_simp_tac (srw_ss()) [FUN_EQ_THM, fnpm_def] >> gen_tac >>
+        ih_commute_tac lhs >> asm_simp_tac (srw_ss()) [pmact_sing_inv] >>
+        disch_then match_mp_tac >>
+        fsrw_tac [][MEM_listpm_EXISTS, gtmsize_gtpm] >>
+        metis_tac [gtmsize_GLAM_subterm, genind_GLAM_subterm]) >>
+  reverse conj_tac >- (
   match_mp_tac supp_fresh >>
   reverse conj_tac >- (
     fsrw_tac [][FCB_def,Abbr‘RHS’] >>
@@ -1239,8 +1206,8 @@ reverse conj_tac >- (
   match_mp_tac notinsupp_I >>
   qunabbrev_tac ‘RHS’ >>
   qexists_tac
-     ‘A ∪ {s''} ∪ supp ppm (pmact ppm [(x,y)] p) ∪
-      set (listpm string_pmact [(x,y)] fvs) ∪ GFVl xyus ∪ GFVl usxyts’ >>
+  ‘A ∪ {s''} ∪ supp ppm (pmact ppm [(x,y)] p) ∪
+   set (listpm string_pmact [(x,y)] fvs) ∪ GFVl xyus ∪ GFVl usxyts’ >>
   ‘FINITE A ∧ (∀p. FINITE (supp ppm p))’ by fsrw_tac [][sidecond_def] >>
   asm_simp_tac (srw_ss()) [support_def] >> reverse conj_tac
   >- simp[MEM_listpm, Abbr‘u’] >>
@@ -1266,28 +1233,28 @@ reverse conj_tac >- (
   map_every qunabbrev_tac [‘usxyts’, ‘xyus’] >>
   fsrw_tac [][MEM_listpm_EXISTS, gtmsize_gtpm] >>
   metis_tac [gtmsize_GLAM_subterm, genind_GLAM_subterm]) >>
-srw_tac [][Abbr‘RHS’] >>
-sidecond_tac rhs >> impl_tac >- simp[genind_ignores_fvspm] >>
-asm_simp_tac (srw_ss()) [listpm_tMAP, supp_fresh] >>
-disch_then (K ALL_TAC) >>
-qunabbrev_tac ‘LHS’ >> rpt AP_THM_TAC >>
-qunabbrev_tac ‘usxyts’ >>
-asm_simp_tac (srw_ss() ++ ETA_ss) [pmact_sing_inv, pmact_nil] >>
-AP_THM_TAC >>
-qmatch_abbrev_tac ‘lf u FVS1 bv X1 Y1 = lf u FVS2 bv X2 Y2’ >>
-qsuff_tac ‘FVS1 = FVS2 ∧ X1 = X2 ∧ Y1 = Y2’ >- srw_tac [][] >>
-map_every qunabbrev_tac [‘X1’,‘X2’,‘Y1’, ‘Y2’, ‘FVS1’, ‘FVS2’] >>
-conj_tac
->- (simp[Abbr‘usxyfvs’] >> sym_tac >> irule supp_fresh >>
-    simp[IN_supp_listpm] >> simp[MEM_listpm, Abbr‘u’]) >>
-conj_tac >> (* splits in two *)
-srw_tac [][MAP_EQ_f, FUN_EQ_THM, fnpm_def] >>
-ih_commute_tac rhs >>
-asm_simp_tac (srw_ss()) [pmact_sing_inv, gtmsize_gtpm] >>
-disch_then (match_mp_tac o GSYM) >>
-qunabbrev_tac ‘xyus’ >>
-fsrw_tac [][MEM_listpm_EXISTS, gtmsize_gtpm] >>
-metis_tac [genind_GLAM_subterm, gtmsize_GLAM_subterm]
+  srw_tac [][Abbr‘RHS’] >>
+  sidecond_tac rhs >> impl_tac >- simp[genind_ignores_fvspm] >>
+  asm_simp_tac (srw_ss()) [listpm_tMAP, supp_fresh] >>
+  disch_then (K ALL_TAC) >>
+  qunabbrev_tac ‘LHS’ >> rpt AP_THM_TAC >>
+  qunabbrev_tac ‘usxyts’ >>
+  asm_simp_tac (srw_ss() ++ ETA_ss) [pmact_sing_inv, pmact_nil] >>
+  AP_THM_TAC >>
+  qmatch_abbrev_tac ‘lf u FVS1 bv X1 Y1 = lf u FVS2 bv X2 Y2’ >>
+  qsuff_tac ‘FVS1 = FVS2 ∧ X1 = X2 ∧ Y1 = Y2’ >- srw_tac [][] >>
+  map_every qunabbrev_tac [‘X1’,‘X2’,‘Y1’, ‘Y2’, ‘FVS1’, ‘FVS2’] >>
+  conj_tac
+  >- (simp[Abbr‘usxyfvs’] >> sym_tac >> irule supp_fresh >>
+      simp[IN_supp_listpm] >> simp[MEM_listpm, Abbr‘u’]) >>
+  conj_tac >> (* splits in two *)
+  srw_tac [][MAP_EQ_f, FUN_EQ_THM, fnpm_def] >>
+  ih_commute_tac rhs >>
+  asm_simp_tac (srw_ss()) [pmact_sing_inv, gtmsize_gtpm] >>
+  disch_then (match_mp_tac o GSYM) >>
+  qunabbrev_tac ‘xyus’ >>
+  fsrw_tac [][MEM_listpm_EXISTS, gtmsize_gtpm] >>
+  metis_tac [genind_GLAM_subterm, gtmsize_GLAM_subterm]
 QED
 
 fun udplus th =
@@ -1297,24 +1264,25 @@ fun udplus th =
 
 val eqv_I = tmrec_equivariant |> udplus
 
-val tmrec_fresh = store_thm(
-  "tmrec_fresh",
-  ``sidecond dpm ppm A ^vp ^lp ^vf ^lf ∧ FCB dpm ppm A vp lp lf ==>
-    ∀n t. genind vp lp n t ==>
+Theorem tmrec_fresh:
+  sidecond dpm ppm A ^lp ^lf ∧ FCB dpm ppm A lp lf ==>
+    ∀n t. genind lp n t ==>
           ∀x. x ∉ A ∧ x ∉ GFV t ==>
-              x ∉ supp (fn_pmact ppm dpm) (tmrec A ppm vf lf t)``,
+              x ∉ supp (fn_pmact ppm dpm) (tmrec A ppm lf t)
+Proof
   srw_tac [][] >> match_mp_tac notinsupp_I >> qexists_tac `GFV t ∪ A` >>
   `FINITE A` by fsrw_tac [][sidecond_def] >>
   srw_tac [][support_def, FUN_EQ_THM, fnpm_def] >>
-  metis_tac [tmrec_equivariant, supp_fresh, pmact_sing_inv]);
+  metis_tac [tmrec_equivariant, supp_fresh, pmact_sing_inv]
+QED
 
 Definition NEWFCB_def:
-  NEWFCB dpm ppm A vp lp lf ⇔
+  NEWFCB dpm ppm A lp lf ⇔
   ∀a1 a2 n fvs bv r1 r2 ts us p.
      a1 ∉ A ∧ a1 ∉ supp ppm p ∧ a2 ∉ A ∧ a2 ∉ GFVl ts ∧ a2 ∉ supp ppm p ∧
      LIST_REL (relsupp A dpm ppm) ts r1 ∧
      LIST_REL (relsupp A dpm ppm) us r2 ∧
-     genind vp lp n (GLAM a1 fvs bv ts us) ==>
+     genind lp n (GLAM a1 fvs bv ts us) ==>
      (lf a2 fvs bv (listpm (fn_pmact ppm dpm) [(a2,a1)] r1) r2
                (gtpml [(a2,a1)] ts) us p =
       lf a1 fvs bv r1 r2 ts us p)
@@ -1332,8 +1300,8 @@ Proof
 QED
 
 Theorem NEWFCB_OLD:
-  NEWFCB dpm ppm A vp lp ^lf ∧ sidecond dpm ppm A vp lp vf lf ==>
-  FCB dpm ppm A vp lp lf
+  NEWFCB dpm ppm A lp ^lf ∧ sidecond dpm ppm A lp lf ==>
+  FCB dpm ppm A lp lf
 Proof
   srw_tac [][FCB_def, NEWFCB_def] >>
   ‘FINITE A ∧ (∀p. FINITE (supp ppm p))’
@@ -1378,24 +1346,22 @@ fun xmatch_cond_assum dir (asl,w) =
                           (dir w))) (asl,w)
 
 Theorem parameter_gtm_recursion:
-  sidecond dpm ppm A ^vp ^lp ^vf ^lf ∧ NEWFCB dpm ppm A ^vp ^lp ^lf ⇒
+  sidecond dpm ppm A ^lp ^lf ∧ NEWFCB dpm ppm A ^lp ^lf ⇒
   ∃f.
-    ((∀n s vv p. genind vp lp n (GVAR s vv) ⇒ (f (GVAR s vv) p = vf s vv p)) ∧
-     ∀n v fvs bv ns ms ts us p.
-       v ∉ A ∧ v ∉ supp ppm p ∧ genind vp lp n (GLAM v fvs bv ts us) ⇒
+    (∀n v fvs bv ns ms ts us p.
+       v ∉ A ∧ v ∉ supp ppm p ∧ genind lp n (GLAM v fvs bv ts us) ⇒
        (f (GLAM v fvs bv ts us) p = lf v fvs bv (MAP f ts) (MAP f us) ts us p)) ∧
     ∀n t p.
-      genind vp lp n t ==>
+      genind lp n t ==>
       ∀x y. x ∉ A ∧ y ∉ A ==>
             pmact dpm [(x,y)] (f t p) =
             f (gtpm [(x,y)] t) (pmact ppm [(x,y)] p)
 Proof
   strip_tac >>
   ‘FINITE A ∧ ∀p. FINITE (supp ppm p)’ by fsrw_tac [][sidecond_def] >>
-  qexists_tac ‘tmrec A ppm vf lf’ >>
+  qexists_tac ‘tmrec A ppm lf’ >>
   reverse conj_tac
   >- (rpt strip_tac >> imp_res_tac eqv_I >> srw_tac [][]) >>
-  conj_tac >- srw_tac [][tmrec_GVAR] >>
   srw_tac [][tmrec_GLAM] >>
   DEEP_INTRO_TAC optionTheory.some_intro >>
   asm_simp_tac (srw_ss()) [pairTheory.FORALL_PROD, pairTheory.EXISTS_PROD] >>
@@ -1409,8 +1375,8 @@ Proof
       metis_tac []) >>
   asm_simp_tac (srw_ss()++DNF_ss++ETA_ss) [GLAM_eq_thm,gtpml_eqr,gtpm_eqr] >>
   qx_gen_tac ‘u’ >> strip_tac >>
-  ‘LIST_REL (relsupp A dpm ppm) ts (MAP (tmrec A ppm vf lf) ts) ∧
-   LIST_REL (relsupp A dpm ppm) us (MAP (tmrec A ppm vf lf) us)’
+  ‘LIST_REL (relsupp A dpm ppm) ts (MAP (tmrec A ppm lf) ts) ∧
+   LIST_REL (relsupp A dpm ppm) us (MAP (tmrec A ppm lf) us)’
     by (assume_tac fresh_I >>
         fsrw_tac [DNF_ss][MEM_EL] >>
         srw_tac [][LIST_REL_EL_EQN, EL_MAP, relsupp_def] >>
@@ -1421,8 +1387,8 @@ Proof
         srw_tac [][MEM_EL] >>
         metis_tac []) >>
   asm_simp_tac (srw_ss()) [pmact_flip_args] >>
-  qsuff_tac ‘MAP (tmrec A ppm vf lf) (gtpml [(u,v)] ts) =
-             listpm (fn_pmact ppm dpm) [(u,v)] (MAP (tmrec A ppm vf lf) ts)’
+  qsuff_tac ‘MAP (tmrec A ppm lf) (gtpml [(u,v)] ts) =
+             listpm (fn_pmact ppm dpm) [(u,v)] (MAP (tmrec A ppm lf) ts)’
   >- (disch_then SUBST1_TAC >> fsrw_tac [][NEWFCB_def] >>
       first_x_assum match_mp_tac >> fsrw_tac [][perm_supp] >> metis_tac []) >>
   srw_tac [][listpm_tMAP, MAP_EQ_f, MEM_listpm_EXISTS, FUN_EQ_THM, fnpm_def] >>
