examples/lambda/basics/termScript.sml
@@ -19,21 +19,22 @@ val _ = set_fixity "=" (Infix(NONASSOC, 450))
 
 val tyname = "term"
 
-val vp = “(λn u:unit. n = 0)”
-val lp = “(λn lfvs (d:unit + unit) tns uns.
-             lfvs = 0 ∧ n = 0 ∧ ISL d ∧ tns = [] ∧ uns = [0;0] ∨
-             lfvs = 0 ∧ n = 0 ∧ ISR d ∧ tns = [0] ∧ uns = [])”
+(* d ≈ var + app + lam *)
+val lp = “(λn lfvs (d:unit + unit + unit) tns uns.
+             lfvs = 1 ∧ n = 0 ∧ ISL d ∧ tns = [] ∧ uns = [] ∨
+             lfvs = 0 ∧ n = 0 ∧ ISR d ∧ ISL (OUTR d) ∧ tns = [] ∧ uns = [0;0] ∨
+             lfvs = 0 ∧ n = 0 ∧ ISR d ∧ ISR (OUTR d) ∧ tns = [0] ∧ uns = [])”
 
 val {term_ABS_pseudo11, term_REP_11, genind_term_REP, genind_exists,
      termP, absrep_id, repabs_pseudo_id, term_REP_t, term_ABS_t, newty, ...} =
-    new_type_step1 tyname 0 [] {vp = vp, lp = lp};
+    new_type_step1 tyname 0 [] {lp = lp};
 
-val [gvar,glam] = genind_rules |> SPEC_ALL |> CONJUNCTS
+val glam = genind_lam
 
 val LAM_t = mk_var("LAM", ``:string -> ^newty -> ^newty``)
 val LAM_def = new_definition(
   "LAM_def",
-  ``^LAM_t v t = ^term_ABS_t (GLAM v [] (INR ()) [^term_REP_t t] [])``);
+  ``^LAM_t v t = ^term_ABS_t (GLAM v [] (INR $ INR ()) [^term_REP_t t] [])``);
 
 val LAM_termP = prove(
   mk_comb(termP, LAM_def |> SPEC_ALL |> concl |> rhs |> rand),
@@ -44,14 +45,15 @@ val APP_t = mk_var("APP", ``:^newty -> ^newty -> ^newty``)
 val APP_def = new_definition(
   "APP_def",
   ``^APP_t t1 t2 =
-       ^term_ABS_t (GLAM ARB [] (INL ()) [] [^term_REP_t t1; ^term_REP_t t2])``);
+       ^term_ABS_t (GLAM ARB [] (INR $ INL ()) []
+                         [^term_REP_t t1; ^term_REP_t t2])``);
 val APP_termP = prove(
-  ``^termP (GLAM x [] (INL ()) [] [^term_REP_t t1; ^term_REP_t t2])``,
+  ``^termP (GLAM x [] (INR $ INL ()) [] [^term_REP_t t1; ^term_REP_t t2])``,
   match_mp_tac glam >> srw_tac [][genind_term_REP])
 val APP_t = defined_const APP_def
 
 Theorem APP_def':
-  ^term_ABS_t (GLAM v [] (INL ()) [] [^term_REP_t t1; ^term_REP_t t2]) =
+  ^term_ABS_t (GLAM v [] (INR $ INL ()) [] [^term_REP_t t1; ^term_REP_t t2]) =
   ^APP_t t1 t2
 Proof srw_tac [][APP_def, GLAM_NIL_EQ, term_ABS_pseudo11, APP_termP]
 QED
@@ -59,14 +61,21 @@ QED
 val VAR_t = mk_var("VAR", ``:string -> ^newty``)
 val VAR_def = new_definition(
   "VAR_def",
-  ``^VAR_t s = ^term_ABS_t (GVAR s ())``);
-val VAR_termP = prove(
-  mk_comb(termP, VAR_def |> SPEC_ALL |> concl |> rhs |> rand),
-  srw_tac [][genind_rules]);
+  ``^VAR_t s = ^term_ABS_t (GLAM ARB [s] (INL ()) [] [])``);
+Theorem VAR_termP[local]:
+  ^termP (GLAM u [v] (INL ()) [][])
+Proof irule glam >> srw_tac[][genind_term_REP]
+QED
 val VAR_t = defined_const VAR_def
 
+Theorem VAR_def':
+  ^term_ABS_t (GLAM u [v] (INL ()) [] []) = ^VAR_t v
+Proof
+  srw_tac[][VAR_def, GLAM_NIL_EQ, term_ABS_pseudo11, VAR_termP]
+QED
+
 val cons_info =
-    [{con_termP = VAR_termP, con_def = VAR_def},
+    [{con_termP = VAR_termP, con_def = SYM VAR_def'},
      {con_termP = APP_termP, con_def = SYM APP_def'},
      {con_termP = LAM_termP, con_def = LAM_def}]
 
@@ -127,7 +136,7 @@ fun supp_clause {con_termP, con_def} = let
 in
   t |> REWRITE_CONV [supp_tpm, con_def, MATCH_MP repabs_pseudo_id con_termP,
                      GFV_thm]
-    |> REWRITE_RULE [supp_listpm, EMPTY_DELETE, UNION_EMPTY]
+    |> REWRITE_RULE [supp_listpm, EMPTY_DELETE, UNION_EMPTY, LIST_TO_SET_THM]
     |> REWRITE_RULE [GSYM supp_tpm]
     |> GEN_ALL
 end
@@ -151,8 +160,8 @@ val LIST_REL_NIL = listTheory.LIST_REL_NIL
 
 val term_ind =
     bvc_genind
-        |> INST_TYPE [alpha |-> ``:unit+unit``, beta |-> ``:unit``]
-        |> Q.INST [`vp` |-> `^vp`, `lp` |-> `^lp`]
+        |> INST_TYPE [alpha |-> ``:unit+unit+unit``]
+        |> Q.INST [`lp` |-> `^lp`]
         |> SIMP_RULE std_ss [LIST_REL_CONS1, RIGHT_AND_OVER_OR,
                              LEFT_AND_OVER_OR, DISJ_IMP_THM, LIST_REL_NIL]
         |> Q.SPEC `λn t0 x. Q t0 x`
@@ -160,14 +169,15 @@ val term_ind =
         |> UNDISCH |> Q.SPEC `0` |> DISCH_ALL
         |> SIMP_RULE (std_ss ++ DNF_ss)
                      [sumTheory.FORALL_SUM, supp_listpm,
+                      LENGTH_EQ_NUM_compute,
                       IN_UNION, NOT_IN_EMPTY, oneTheory.FORALL_ONE,
                       genind_exists, LIST_REL_CONS1, LIST_REL_NIL]
         |> Q.INST [`Q` |-> `λt. P (term_ABS t)`]
-        |> SIMP_RULE std_ss [GSYM LAM_def, APP_def', GSYM VAR_def, absrep_id,
+        |> SIMP_RULE std_ss [GSYM LAM_def, APP_def', VAR_def', absrep_id,
                              LENGTH_NIL]
         |> SIMP_RULE (srw_ss()) [GSYM supp_tpm]
         |> elim_unnecessary_atoms {finite_fv = FINITE_FV}
-                                  [ASSUME ``!x:'c. FINITE (fv x:string set)``]
+                                  [ASSUME ``!x:'b. FINITE (fv x:string set)``]
         |> SPEC_ALL |> UNDISCH
         |> genit |> DISCH_ALL |> Q.GEN `fv` |> Q.GEN `P`
 
@@ -205,13 +215,16 @@ val (_, repty) = dom_rng (type_of term_REP_t)
 val repty' = ty_antiq repty
 
 val tlf =
-   “λ(v:string) (fvs : string list) (u:unit + unit)
+   “λ(v:string) (fvs : string list) (u:unit + unit + unit)
      (ds1:(ρ -> α) list) (ds2:(ρ -> α) list)
      (ts1:^repty' list) (ts2:^repty' list) (p :ρ).
-       if ISR u then tlf (HD ds1) v (^term_ABS_t (HD ts1)) p :α
-       else taf (HD ds2) (HD (TL ds2)) (^term_ABS_t (HD ts2))
-                (^term_ABS_t (HD (TL ts2))) p :α”
-val tvf = “λ(s:string) (u:unit) (p:ρ). tvf s p :α”;
+      if ISL u then
+        tvf (HD fvs) p
+      else if ISL (OUTR u) then
+        taf (HD ds2) (HD (TL ds2)) (^term_ABS_t (HD ts2))
+            (^term_ABS_t (HD (TL ts2))) p :α
+      else
+        tlf (HD ds1) v (^term_ABS_t (HD ts1)) p :α”
 
 val termP_elim = prove(
   ``(∀g. ^termP g ⇒ P g) ⇔ (∀t. P (^term_REP_t t))``,
@@ -226,26 +239,24 @@ val termP_removal =
       termP = termP, repty = repty}
 
 val termP0 = prove(
-  ``genind ^vp ^lp n t <=> ^termP t ∧ (n = 0)``,
+  ``genind ^lp n t <=> ^termP t ∧ (n = 0)``,
   EQ_TAC >> simp_tac (srw_ss()) [] >> strip_tac >>
   qsuff_tac `n = 0` >- (strip_tac >> srw_tac [][]) >>
   pop_assum mp_tac >>
   Q.ISPEC_THEN `t` STRUCT_CASES_TAC gterm_cases >>
-  srw_tac [][genind_GVAR, genind_GLAM_eqn]);
+  srw_tac [][genind_GLAM_eqn]);
 
-val parameter_tm_recursion = save_thm(
-  "parameter_tm_recursion",
+Theorem parameter_tm_recursion =
   parameter_gtm_recursion
-      |> INST_TYPE [alpha |-> ``:unit + unit``, beta |-> ``:unit``,
+      |> INST_TYPE [alpha |-> ``:unit + unit + unit``,
                     gamma |-> alpha]
-      |> Q.INST [`lf` |-> `^tlf`, `vf` |-> `^tvf`, `vp` |-> `^vp`,
-                 `lp` |-> `^lp`]
+      |> Q.INST [`lf` |-> `^tlf`, `lp` |-> `^lp`]
       |> SIMP_RULE (srw_ss()) [sumTheory.FORALL_SUM, FORALL_AND_THM,
                                GSYM RIGHT_FORALL_IMP_THM, IMP_CONJ_THM,
                                GSYM RIGHT_EXISTS_AND_THM,
                                GSYM LEFT_EXISTS_AND_THM,
                                GSYM LEFT_FORALL_IMP_THM,
-                               LIST_REL_CONS1, genind_GVAR,
+                               LIST_REL_CONS1, LENGTH_EQ_NUM_compute,
                                genind_GLAM_eqn, sidecond_def,
                                NEWFCB_def, relsupp_def,
                                LENGTH_NIL_SYM, LENGTH1, LENGTH2]
@@ -267,7 +278,7 @@ val parameter_tm_recursion = save_thm(
       |> CONV_RULE (LAND_CONV (REWRITE_CONV [GSYM CONJ_ASSOC]))
       |> Q.INST [`tvf` |-> `vr`, `tlf` |-> `lm`, `taf` |-> `ap`,
                  `dpm` |-> `apm`]
-      |> CONV_RULE (REDEPTH_CONV sort_uvars))
+      |> CONV_RULE (REDEPTH_CONV sort_uvars)
 
 val tm_recursion = save_thm(
   "tm_recursion",
@@ -369,7 +380,7 @@ Theorem term_distinct[simp]:
   VAR s ≠ APP t1 t2 ∧ VAR s ≠ LAM v t ∧ APP t1 t2 ≠ LAM v t
 Proof
   srw_tac [][VAR_def, APP_def, LAM_def, LAM_termP, VAR_termP, APP_termP,
-             term_ABS_pseudo11, gterm_distinct, GLAM_eq_thm]
+             term_ABS_pseudo11, GLAM_eq_thm]
 QED
 
 Theorem term_11[simp]:
